transport to 64-bit types

code/mpfr/injected/add1sp1_extracted.c
@@ -1,0 +1,361 @@
+/* mpfr_add1sp1 -- internal function to perform a "real" addition on one limb
+   This code was extracted by Kremlin from a formal proof in F*
+   done by Jianyang Pan in April-August 2018: do not modify it!
+
+Copyright 2004-2018 Free Software Foundation, Inc.
+Contributed by the AriC and Caramba projects, INRIA.
+
+This file is part of the GNU MPFR Library.
+
+The GNU MPFR Library is free software; you can redistribute it and/or modify
+it under the terms of the GNU Lesser General Public License as published by
+the Free Software Foundation; either version 3 of the License, or (at your
+option) any later version.
+
+The GNU MPFR Library is distributed in the hope that it will be useful, but
+WITHOUT ANY WARRANTY; without even the implied warranty of MERCHANTABILITY
+or FITNESS FOR A PARTICULAR PURPOSE.  See the GNU Lesser General Public
+License for more details.
+
+You should have received a copy of the GNU Lesser General Public License
+along with the GNU MPFR Library; see the file COPYING.LESSER.  If not, see
+http://www.gnu.org/licenses/ or write to the Free Software Foundation, Inc.,
+51 Franklin St, Fifth Floor, Boston, MA 02110-1301, USA. */
+
+#define int64_t long
+#define uint32_t unsigned int
+#define uint64_t mp_limb_t
+
+typedef struct MPFR_Add1sp1_state_s
+{
+  int64_t sh;
+  int64_t bx;
+  uint64_t rb;
+  uint64_t sb;
+}
+MPFR_Add1sp1_state;
+
+static MPFR_Add1sp1_state
+MPFR_Add1sp1_mk_state(int64_t sh, int64_t bx, uint64_t rb, uint64_t sb)
+{
+  return ((MPFR_Add1sp1_state){ .sh = sh, .bx = bx, .rb = rb, .sb = sb });
+}
+
+typedef struct K___uint64_t_int64_t_s
+{
+  uint64_t fst;
+  int64_t snd;
+}
+K___uint64_t_int64_t;
+
+typedef struct K___uint64_t_uint64_t_int64_t_s
+{
+  uint64_t fst;
+  uint64_t snd;
+  int64_t thd;
+}
+K___uint64_t_uint64_t_int64_t;
+
+#define MPFR_Lib_mpfr_struct __mpfr_struct
+#define MPFR_Lib_mpfr_RET(I) ((I) != 0 ? ((__gmpfr_flags |= MPFR_FLAGS_INEXACT), (I)) : 0)
+#define MPFR_Exceptions_mpfr_overflow mpfr_overflow
+#define mpfr_prec _mpfr_prec
+#define mpfr_exp _mpfr_exp
+#define mpfr_d _mpfr_d
+#define mpfr_sign _mpfr_sign
+#define MPFR_Lib_gmp_NUMB_BITS GMP_NUMB_BITS
+#define MPFR_Lib_mpfr_EMAX __gmpfr_emax
+
+#define MPFR_RoundingMode_uu___is_MPFR_RNDN(rnd_mode) (rnd_mode == MPFR_RNDN)
+#define MPFR_RoundingMode_mpfr_IS_LIKE_RNDZ MPFR_IS_LIKE_RNDZ
+
+/* same as mpfr_add1sp, but for p < GMP_NUMB_BITS */
+static int
+mpfr_add1sp1 (mpfr_ptr a, mpfr_srcptr b, mpfr_srcptr c, mpfr_rnd_t rnd_mode,
+              mpfr_prec_t p)
+{
+  MPFR_Lib_mpfr_struct a0 = a[0U];
+  MPFR_Lib_mpfr_struct b0 = b[0U];
+  MPFR_Lib_mpfr_struct c0 = c[0U];
+  int64_t bx = b0.mpfr_exp;
+  int64_t cx = c0.mpfr_exp;
+  int64_t sh = MPFR_Lib_gmp_NUMB_BITS - p;
+  MPFR_Add1sp1_state st;
+  if (bx == cx)
+  {
+    uint64_t *ap = a0.mpfr_d;
+    uint64_t *bp = b0.mpfr_d;
+    uint64_t *cp = c0.mpfr_d;
+    uint64_t a01 = (bp[0U] >> (uint32_t)1U) + (cp[0U] >> (uint32_t)1U);
+    int64_t bx1 = b0.mpfr_exp + (int64_t)1;
+    uint64_t rb = a01 & (uint64_t)1U << (uint32_t)(sh - (int64_t)1);
+    ap[0U] = a01 ^ rb;
+    uint64_t sb = (uint64_t)0U;
+    st = MPFR_Add1sp1_mk_state(sh, bx1, rb, sb);
+  }
+  else
+  {
+    MPFR_Add1sp1_state ite0;
+    if (bx > cx)
+    {
+      int64_t bx1 = b0.mpfr_exp;
+      int64_t cx1 = c0.mpfr_exp;
+      int64_t d = bx1 - cx1;
+      uint64_t mask = ((uint64_t)1U << (uint32_t)sh) - (uint64_t)1U;
+      MPFR_Add1sp1_state ite1;
+      if (d < sh)
+      {
+        uint64_t *ap = a0.mpfr_d;
+        uint64_t *bp = b0.mpfr_d;
+        uint64_t *cp = c0.mpfr_d;
+        int64_t bx2 = b0.mpfr_exp;
+        uint64_t a01 = bp[0U] + (cp[0U] >> (uint32_t)d);
+        K___uint64_t_int64_t scrut;
+        if (a01 < bp[0U])
+          scrut =
+            (
+              (K___uint64_t_int64_t){
+                .fst = (uint64_t)0x8000000000000000U | a01 >> (uint32_t)1U,
+                .snd = bx2 + (int64_t)1
+              }
+            );
+        else
+          scrut = ((K___uint64_t_int64_t){ .fst = a01, .snd = bx2 });
+        uint64_t a02 = scrut.fst;
+        int64_t bx3 = scrut.snd;
+        uint64_t rb = a02 & (uint64_t)1U << (uint32_t)(sh - (int64_t)1);
+        uint64_t sb = (a02 & mask) ^ rb;
+        ap[0U] = a02 & ~mask;
+        ite1 = MPFR_Add1sp1_mk_state(sh, bx3, rb, sb);
+      }
+      else
+      {
+        MPFR_Add1sp1_state ite;
+        if (d < MPFR_Lib_gmp_NUMB_BITS)
+        {
+          uint64_t *ap = a0.mpfr_d;
+          uint64_t *bp = b0.mpfr_d;
+          uint64_t *cp = c0.mpfr_d;
+          int64_t bx2 = b0.mpfr_exp;
+          uint64_t sb = cp[0U] << (uint32_t)(MPFR_Lib_gmp_NUMB_BITS - d);
+          uint64_t a01 = bp[0U] + (cp[0U] >> (uint32_t)d);
+          K___uint64_t_uint64_t_int64_t scrut;
+          if (a01 < bp[0U])
+            scrut =
+              (
+                (K___uint64_t_uint64_t_int64_t){
+                  .fst = sb | (a01 & (uint64_t)1U),
+                  .snd = (uint64_t)0x8000000000000000U | a01 >> (uint32_t)1U,
+                  .thd = bx2 + (int64_t)1
+                }
+              );
+          else
+            scrut = ((K___uint64_t_uint64_t_int64_t){ .fst = sb, .snd = a01, .thd = bx2 });
+          uint64_t sb1 = scrut.fst;
+          uint64_t a02 = scrut.snd;
+          int64_t bx3 = scrut.thd;
+          uint64_t rb = a02 & (uint64_t)1U << (uint32_t)(sh - (int64_t)1);
+          uint64_t sb2 = sb1 | ((a02 & mask) ^ rb);
+          ap[0U] = a02 & ~mask;
+          ite = MPFR_Add1sp1_mk_state(sh, bx3, rb, sb2);
+        }
+        else
+        {
+          uint64_t *ap = a0.mpfr_d;
+          uint64_t *bp = b0.mpfr_d;
+          int64_t bx2 = b0.mpfr_exp;
+          ap[0U] = bp[0U];
+          uint64_t rb = (uint64_t)0U;
+          uint64_t sb = (uint64_t)1U;
+          ite = MPFR_Add1sp1_mk_state(sh, bx2, rb, sb);
+        }
+        ite1 = ite;
+      }
+      ite0 = ite1;
+    }
+    else
+    {
+      int64_t bx1 = c0.mpfr_exp;
+      int64_t cx1 = b0.mpfr_exp;
+      int64_t d = bx1 - cx1;
+      uint64_t mask = ((uint64_t)1U << (uint32_t)sh) - (uint64_t)1U;
+      MPFR_Add1sp1_state ite1;
+      if (d < sh)
+      {
+        uint64_t *ap = a0.mpfr_d;
+        uint64_t *bp = c0.mpfr_d;
+        uint64_t *cp = b0.mpfr_d;
+        int64_t bx2 = c0.mpfr_exp;
+        uint64_t a01 = bp[0U] + (cp[0U] >> (uint32_t)d);
+        K___uint64_t_int64_t scrut;
+        if (a01 < bp[0U])
+          scrut =
+            (
+              (K___uint64_t_int64_t){
+                .fst = (uint64_t)0x8000000000000000U | a01 >> (uint32_t)1U,
+                .snd = bx2 + (int64_t)1
+              }
+            );
+        else
+          scrut = ((K___uint64_t_int64_t){ .fst = a01, .snd = bx2 });
+        uint64_t a02 = scrut.fst;
+        int64_t bx3 = scrut.snd;
+        uint64_t rb = a02 & (uint64_t)1U << (uint32_t)(sh - (int64_t)1);
+        uint64_t sb = (a02 & mask) ^ rb;
+        ap[0U] = a02 & ~mask;
+        ite1 = MPFR_Add1sp1_mk_state(sh, bx3, rb, sb);
+      }
+      else
+      {
+        MPFR_Add1sp1_state ite;
+        if (d < MPFR_Lib_gmp_NUMB_BITS)
+        {
+          uint64_t *ap = a0.mpfr_d;
+          uint64_t *bp = c0.mpfr_d;
+          uint64_t *cp = b0.mpfr_d;
+          int64_t bx2 = c0.mpfr_exp;
+          uint64_t sb = cp[0U] << (uint32_t)(MPFR_Lib_gmp_NUMB_BITS - d);
+          uint64_t a01 = bp[0U] + (cp[0U] >> (uint32_t)d);
+          K___uint64_t_uint64_t_int64_t scrut;
+          if (a01 < bp[0U])
+            scrut =
+              (
+                (K___uint64_t_uint64_t_int64_t){
+                  .fst = sb | (a01 & (uint64_t)1U),
+                  .snd = (uint64_t)0x8000000000000000U | a01 >> (uint32_t)1U,
+                  .thd = bx2 + (int64_t)1
+                }
+              );
+          else
+            scrut = ((K___uint64_t_uint64_t_int64_t){ .fst = sb, .snd = a01, .thd = bx2 });
+          uint64_t sb1 = scrut.fst;
+          uint64_t a02 = scrut.snd;
+          int64_t bx3 = scrut.thd;
+          uint64_t rb = a02 & (uint64_t)1U << (uint32_t)(sh - (int64_t)1);
+          uint64_t sb2 = sb1 | ((a02 & mask) ^ rb);
+          ap[0U] = a02 & ~mask;
+          ite = MPFR_Add1sp1_mk_state(sh, bx3, rb, sb2);
+        }
+        else
+        {
+          uint64_t *ap = a0.mpfr_d;
+          uint64_t *bp = c0.mpfr_d;
+          int64_t bx2 = c0.mpfr_exp;
+          ap[0U] = bp[0U];
+          uint64_t rb = (uint64_t)0U;
+          uint64_t sb = (uint64_t)1U;
+          ite = MPFR_Add1sp1_mk_state(sh, bx2, rb, sb);
+        }
+        ite1 = ite;
+      }
+      ite0 = ite1;
+    }
+    st = ite0;
+  }
+  if (st.bx > MPFR_Lib_mpfr_EMAX)
+  {
+    int32_t t = MPFR_Exceptions_mpfr_overflow(a, rnd_mode, a->mpfr_sign);
+    return t;
+  }
+  else
+  {
+    uint64_t *ap = a->mpfr_d;
+    uint64_t a01 = ap[0U];
+    MPFR_Lib_mpfr_struct uu___72_3478 = a[0U];
+    a[0U] =
+      (
+        (MPFR_Lib_mpfr_struct){
+          .mpfr_prec = uu___72_3478.mpfr_prec,
+          .mpfr_sign = uu___72_3478.mpfr_sign,
+          .mpfr_exp = st.bx,
+          .mpfr_d = uu___72_3478.mpfr_d
+        }
+      );
+    if (st.rb == (uint64_t)0U && st.sb == (uint64_t)0U)
+      return MPFR_Lib_mpfr_RET((int32_t)0);
+    else if (MPFR_RoundingMode_uu___is_MPFR_RNDN(rnd_mode))
+      if
+      (
+        st.rb
+        == (uint64_t)0U
+        || (st.sb == (uint64_t)0U && (a01 & (uint64_t)1U << (uint32_t)st.sh) == (uint64_t)0U)
+      )
+      {
+        int32_t ite;
+        if (a->mpfr_sign == (int32_t)1)
+          ite = (int32_t)-1;
+        else
+          ite = (int32_t)1;
+        return MPFR_Lib_mpfr_RET(ite);
+      }
+      else
+      {
+        uint64_t *ap1 = a->mpfr_d;
+        ap1[0U] = ap1[0U] + ((uint64_t)1U << (uint32_t)st.sh);
+        if (ap1[0U] == (uint64_t)0U)
+        {
+          ap1[0U] = (uint64_t)0x8000000000000000U;
+          if (st.bx + (int64_t)1 <= MPFR_Lib_mpfr_EMAX)
+          {
+            MPFR_Lib_mpfr_struct uu___72_3574 = a[0U];
+            a[0U] =
+              (
+                (MPFR_Lib_mpfr_struct){
+                  .mpfr_prec = uu___72_3574.mpfr_prec,
+                  .mpfr_sign = uu___72_3574.mpfr_sign,
+                  .mpfr_exp = st.bx + (int64_t)1,
+                  .mpfr_d = uu___72_3574.mpfr_d
+                }
+              );
+            return MPFR_Lib_mpfr_RET(a->mpfr_sign);
+          }
+          else
+          {
+            int32_t t = MPFR_Exceptions_mpfr_overflow(a, rnd_mode, a->mpfr_sign);
+            return MPFR_Lib_mpfr_RET(t);
+          }
+        }
+        else
+          return MPFR_Lib_mpfr_RET(a->mpfr_sign);
+      }
+    else if (MPFR_RoundingMode_mpfr_IS_LIKE_RNDZ(rnd_mode, a->mpfr_sign < (int32_t)0))
+    {
+      int32_t ite;
+      if (a->mpfr_sign == (int32_t)1)
+        ite = (int32_t)-1;
+      else
+        ite = (int32_t)1;
+      return MPFR_Lib_mpfr_RET(ite);
+    }
+    else
+    {
+      uint64_t *ap1 = a->mpfr_d;
+      ap1[0U] = ap1[0U] + ((uint64_t)1U << (uint32_t)st.sh);
+      if (ap1[0U] == (uint64_t)0U)
+      {
+        ap1[0U] = (uint64_t)0x8000000000000000U;
+        if (st.bx + (int64_t)1 <= MPFR_Lib_mpfr_EMAX)
+        {
+          MPFR_Lib_mpfr_struct uu___72_3781 = a[0U];
+          a[0U] =
+            (
+              (MPFR_Lib_mpfr_struct){
+                .mpfr_prec = uu___72_3781.mpfr_prec,
+                .mpfr_sign = uu___72_3781.mpfr_sign,
+                .mpfr_exp = st.bx + (int64_t)1,
+                .mpfr_d = uu___72_3781.mpfr_d
+              }
+            );
+          return MPFR_Lib_mpfr_RET(a->mpfr_sign);
+        }
+        else
+        {
+          int32_t t = MPFR_Exceptions_mpfr_overflow(a, rnd_mode, a->mpfr_sign);
+          return MPFR_Lib_mpfr_RET(t);
+        }
+      }
+      else
+        return MPFR_Lib_mpfr_RET(a->mpfr_sign);
+    }
+  }
+}
