code/mpfr/mpfr-c/MPFR.c
@@ -103,18 +103,22 @@ static bool MPFR_RoundingMode_mpfr_IS_LIKE_RNDA(MPFR_RoundingMode_mpfr_rnd_t rnd
     || (MPFR_RoundingMode_uu___is_MPFR_RNDD(rnd) && !neg);
 }
 
-static uint32_t MPFR_Lib_gmp_NUMB_BITS = (uint32_t)64U;
+static int64_t MPFR_Lib_gmp_NUMB_BITS = (int64_t)64;
 
-static int32_t MPFR_Lib_mpfr_EMIN = (int32_t)1 - (int32_t)0x40000000;
+static int64_t MPFR_Lib_mpfr_EXP_ZERO = (int64_t)-0x7fffffffffffffff;
 
-static int32_t MPFR_Lib_mpfr_EMAX = (int32_t)0x40000000 - (int32_t)1;
+static int64_t MPFR_Lib_mpfr_EXP_INF = (int64_t)-0x7ffffffffffffffd;
 
-static void MPFR_Lib_mpn_ZERO(uint64_t *b, uint32_t l)
+static int64_t MPFR_Lib_mpfr_EMIN = (int64_t)-0x3fffffffffffffff;
+
+static int64_t MPFR_Lib_mpfr_EMAX = (int64_t)0x3fffffffffffffff;
+
+static void MPFR_Lib_mpn_ZERO(uint64_t *b, int64_t l)
 {
-  if (!(l == (uint32_t)0U))
+  if (!(l == (int64_t)0))
   {
-    b[l - (uint32_t)1U] = (uint64_t)0U;
-    MPFR_Lib_mpn_ZERO(b, l - (uint32_t)1U);
+    b[(uint32_t)(l - (int64_t)1)] = (uint64_t)0U;
+    MPFR_Lib_mpn_ZERO(b, l - (int64_t)1);
   }
 }
 
@@ -123,56 +127,56 @@ static int32_t MPFR_Lib_mpfr_RET(int32_t t)
   return t;
 }
 
-static void MPFR_Lib_mpfr_setmax_rec(MPFR_Lib_mpfr_struct *x, uint32_t i)
+static void MPFR_Lib_mpfr_setmax_rec(MPFR_Lib_mpfr_struct *x, int64_t i)
 {
   uint64_t *mant = x->mpfr_d;
-  if (i == (uint32_t)0U)
+  if (i == (int64_t)0)
   {
     MPFR_Lib_mpfr_struct f0 = x[0U];
-    uint32_t p = f0.mpfr_prec;
+    int64_t p = f0.mpfr_prec;
     MPFR_Lib_mpfr_struct f = x[0U];
-    uint32_t l = (f.mpfr_prec - (uint32_t)1U) / MPFR_Lib_gmp_NUMB_BITS + (uint32_t)1U;
-    mant[i] = (uint64_t)0xffffffffffffffffU << (l * MPFR_Lib_gmp_NUMB_BITS - p);
+    int64_t l = (f.mpfr_prec - (int64_t)1) / MPFR_Lib_gmp_NUMB_BITS + (int64_t)1;
+    mant[(uint32_t)i] = (uint64_t)0xffffffffffffffffU << (uint32_t)(l * MPFR_Lib_gmp_NUMB_BITS - p);
   }
   else
   {
-    MPFR_Lib_mpfr_setmax_rec(x, i - (uint32_t)1U);
-    mant[i] = (uint64_t)0xffffffffffffffffU;
+    MPFR_Lib_mpfr_setmax_rec(x, i - (int64_t)1);
+    mant[(uint32_t)i] = (uint64_t)0xffffffffffffffffU;
   }
 }
 
 static void MPFR_Lib_mpfr_setmax(MPFR_Lib_mpfr_struct *x)
 {
-  MPFR_Lib_mpfr_struct uu___62_131220 = x[0U];
+  MPFR_Lib_mpfr_struct uu___72_131181 = x[0U];
   x[0U] =
     (
       (MPFR_Lib_mpfr_struct){
-        .mpfr_prec = uu___62_131220.mpfr_prec,
-        .mpfr_sign = uu___62_131220.mpfr_sign,
+        .mpfr_prec = uu___72_131181.mpfr_prec,
+        .mpfr_sign = uu___72_131181.mpfr_sign,
         .mpfr_exp = MPFR_Lib_mpfr_EMAX,
-        .mpfr_d = uu___62_131220.mpfr_d
+        .mpfr_d = uu___72_131181.mpfr_d
       }
     );
   MPFR_Lib_mpfr_struct f = x[0U];
-  MPFR_Lib_mpfr_setmax_rec(x, (f.mpfr_prec - (uint32_t)1U) / MPFR_Lib_gmp_NUMB_BITS);
+  MPFR_Lib_mpfr_setmax_rec(x, (f.mpfr_prec - (int64_t)1) / MPFR_Lib_gmp_NUMB_BITS);
 }
 
 static void MPFR_Lib_mpfr_setmin(MPFR_Lib_mpfr_struct *x)
 {
-  MPFR_Lib_mpfr_struct uu___62_131431 = x[0U];
+  MPFR_Lib_mpfr_struct uu___72_131392 = x[0U];
   x[0U] =
     (
       (MPFR_Lib_mpfr_struct){
-        .mpfr_prec = uu___62_131431.mpfr_prec,
-        .mpfr_sign = uu___62_131431.mpfr_sign,
+        .mpfr_prec = uu___72_131392.mpfr_prec,
+        .mpfr_sign = uu___72_131392.mpfr_sign,
         .mpfr_exp = MPFR_Lib_mpfr_EMIN,
-        .mpfr_d = uu___62_131431.mpfr_d
+        .mpfr_d = uu___72_131392.mpfr_d
       }
     );
   MPFR_Lib_mpfr_struct f = x[0U];
-  uint32_t xn = (f.mpfr_prec - (uint32_t)1U) / MPFR_Lib_gmp_NUMB_BITS;
+  int64_t xn = (f.mpfr_prec - (int64_t)1) / MPFR_Lib_gmp_NUMB_BITS;
   uint64_t *xp = x->mpfr_d;
-  xp[xn] = (uint64_t)0x8000000000000000U;
+  xp[(uint32_t)xn] = (uint64_t)0x8000000000000000U;
   MPFR_Lib_mpn_ZERO(xp, xn);
 }
 
@@ -183,14 +187,14 @@ MPFR_Exceptions_mpfr_overflow(
   int32_t sign
 )
 {
-  MPFR_Lib_mpfr_struct uu___63_80 = x[0U];
+  MPFR_Lib_mpfr_struct uu___73_79 = x[0U];
   x[0U] =
     (
       (MPFR_Lib_mpfr_struct){
-        .mpfr_prec = uu___63_80.mpfr_prec,
+        .mpfr_prec = uu___73_79.mpfr_prec,
         .mpfr_sign = sign,
-        .mpfr_exp = uu___63_80.mpfr_exp,
-        .mpfr_d = uu___63_80.mpfr_d
+        .mpfr_exp = uu___73_79.mpfr_exp,
+        .mpfr_d = uu___73_79.mpfr_d
       }
     );
   if (MPFR_RoundingMode_mpfr_IS_LIKE_RNDZ(rnd_mode, sign < (int32_t)0))
@@ -203,14 +207,14 @@ MPFR_Exceptions_mpfr_overflow(
   }
   else
   {
-    MPFR_Lib_mpfr_struct uu___62_167 = x[0U];
+    MPFR_Lib_mpfr_struct uu___72_166 = x[0U];
     x[0U] =
       (
         (MPFR_Lib_mpfr_struct){
-          .mpfr_prec = uu___62_167.mpfr_prec,
-          .mpfr_sign = uu___62_167.mpfr_sign,
-          .mpfr_exp = (int32_t)-0x80000000 + (int32_t)3,
-          .mpfr_d = uu___62_167.mpfr_d
+          .mpfr_prec = uu___72_166.mpfr_prec,
+          .mpfr_sign = uu___72_166.mpfr_sign,
+          .mpfr_exp = MPFR_Lib_mpfr_EXP_INF,
+          .mpfr_d = uu___72_166.mpfr_d
         }
       );
     return sign;
@@ -224,26 +228,26 @@ MPFR_Exceptions_mpfr_underflow(
   int32_t sign
 )
 {
-  MPFR_Lib_mpfr_struct uu___63_284 = x[0U];
+  MPFR_Lib_mpfr_struct uu___73_279 = x[0U];
   x[0U] =
     (
       (MPFR_Lib_mpfr_struct){
-        .mpfr_prec = uu___63_284.mpfr_prec,
+        .mpfr_prec = uu___73_279.mpfr_prec,
         .mpfr_sign = sign,
-        .mpfr_exp = uu___63_284.mpfr_exp,
-        .mpfr_d = uu___63_284.mpfr_d
+        .mpfr_exp = uu___73_279.mpfr_exp,
+        .mpfr_d = uu___73_279.mpfr_d
       }
     );
   if (MPFR_RoundingMode_mpfr_IS_LIKE_RNDZ(rnd_mode, sign < (int32_t)0))
   {
-    MPFR_Lib_mpfr_struct uu___62_339 = x[0U];
+    MPFR_Lib_mpfr_struct uu___72_334 = x[0U];
     x[0U] =
       (
         (MPFR_Lib_mpfr_struct){
-          .mpfr_prec = uu___62_339.mpfr_prec,
-          .mpfr_sign = uu___62_339.mpfr_sign,
-          .mpfr_exp = (int32_t)-0x80000000 + (int32_t)1,
-          .mpfr_d = uu___62_339.mpfr_d
+          .mpfr_prec = uu___72_334.mpfr_prec,
+          .mpfr_sign = uu___72_334.mpfr_sign,
+          .mpfr_exp = MPFR_Lib_mpfr_EXP_ZERO,
+          .mpfr_d = uu___72_334.mpfr_d
         }
       );
     if (sign == (int32_t)1)
@@ -260,33 +264,33 @@ MPFR_Exceptions_mpfr_underflow(
 
 typedef struct MPFR_Add1sp1_state_s
 {
-  uint32_t sh;
-  int32_t bx;
+  int64_t sh;
+  int64_t bx;
   uint64_t rb;
   uint64_t sb;
 }
 MPFR_Add1sp1_state;
 
 static MPFR_Add1sp1_state
-MPFR_Add1sp1_mk_state(uint32_t sh, int32_t bx, uint64_t rb, uint64_t sb)
+MPFR_Add1sp1_mk_state(int64_t sh, int64_t bx, uint64_t rb, uint64_t sb)
 {
   return ((MPFR_Add1sp1_state){ .sh = sh, .bx = bx, .rb = rb, .sb = sb });
 }
 
-typedef struct K___uint64_t_int32_t_s
+typedef struct K___uint64_t_int64_t_s
 {
   uint64_t fst;
-  int32_t snd;
+  int64_t snd;
 }
-K___uint64_t_int32_t;
+K___uint64_t_int64_t;
 
-typedef struct K___uint64_t_uint64_t_int32_t_s
+typedef struct K___uint64_t_uint64_t_int64_t_s
 {
   uint64_t fst;
   uint64_t snd;
-  int32_t thd;
+  int64_t thd;
 }
-K___uint64_t_uint64_t_int32_t;
+K___uint64_t_uint64_t_int64_t;
 
 static int32_t
 MPFR_Add1sp1_mpfr_add1sp1(
@@ -294,15 +298,15 @@ MPFR_Add1sp1_mpfr_add1sp1(
   MPFR_Lib_mpfr_struct *b,
   MPFR_Lib_mpfr_struct *c,
   MPFR_RoundingMode_mpfr_rnd_t rnd_mode,
-  uint32_t p
+  int64_t p
 )
 {
   MPFR_Lib_mpfr_struct a0 = a[0U];
   MPFR_Lib_mpfr_struct b0 = b[0U];
   MPFR_Lib_mpfr_struct c0 = c[0U];
-  int32_t bx = b0.mpfr_exp;
-  int32_t cx = c0.mpfr_exp;
-  uint32_t sh = MPFR_Lib_gmp_NUMB_BITS - p;
+  int64_t bx = b0.mpfr_exp;
+  int64_t cx = c0.mpfr_exp;
+  int64_t sh = MPFR_Lib_gmp_NUMB_BITS - p;
   MPFR_Add1sp1_state st;
   if (bx == cx)
   {
@@ -310,8 +314,8 @@ MPFR_Add1sp1_mpfr_add1sp1(
     uint64_t *bp = b0.mpfr_d;
     uint64_t *cp = c0.mpfr_d;
     uint64_t a01 = (bp[0U] >> (uint32_t)1U) + (cp[0U] >> (uint32_t)1U);
-    int32_t bx1 = b0.mpfr_exp + (int32_t)1;
-    uint64_t rb = a01 & (uint64_t)1U << (sh - (uint32_t)1U);
+    int64_t bx1 = b0.mpfr_exp + (int64_t)1;
+    uint64_t rb = a01 & (uint64_t)1U << (uint32_t)(sh - (int64_t)1);
     ap[0U] = a01 ^ rb;
     uint64_t sb = (uint64_t)0U;
     st = MPFR_Add1sp1_mk_state(sh, bx1, rb, sb);
@@ -321,32 +325,32 @@ MPFR_Add1sp1_mpfr_add1sp1(
     MPFR_Add1sp1_state ite0;
     if (bx > cx)
     {
-      int32_t bx1 = b0.mpfr_exp;
-      int32_t cx1 = c0.mpfr_exp;
-      uint32_t d = (uint32_t)(bx1 - cx1);
-      uint64_t mask = ((uint64_t)1U << sh) - (uint64_t)1U;
+      int64_t bx1 = b0.mpfr_exp;
+      int64_t cx1 = c0.mpfr_exp;
+      int64_t d = bx1 - cx1;
+      uint64_t mask = ((uint64_t)1U << (uint32_t)sh) - (uint64_t)1U;
       MPFR_Add1sp1_state ite1;
       if (d < sh)
       {
         uint64_t *ap = a0.mpfr_d;
         uint64_t *bp = b0.mpfr_d;
         uint64_t *cp = c0.mpfr_d;
-        int32_t bx2 = b0.mpfr_exp;
-        uint64_t a01 = bp[0U] + (cp[0U] >> d);
-        K___uint64_t_int32_t scrut;
+        int64_t bx2 = b0.mpfr_exp;
+        uint64_t a01 = bp[0U] + (cp[0U] >> (uint32_t)d);
+        K___uint64_t_int64_t scrut;
         if (a01 < bp[0U])
           scrut =
             (
-              (K___uint64_t_int32_t){
+              (K___uint64_t_int64_t){
                 .fst = (uint64_t)0x8000000000000000U | a01 >> (uint32_t)1U,
-                .snd = bx2 + (int32_t)1
+                .snd = bx2 + (int64_t)1
               }
             );
         else
-          scrut = ((K___uint64_t_int32_t){ .fst = a01, .snd = bx2 });
+          scrut = ((K___uint64_t_int64_t){ .fst = a01, .snd = bx2 });
         uint64_t a02 = scrut.fst;
-        int32_t bx3 = scrut.snd;
-        uint64_t rb = a02 & (uint64_t)1U << (sh - (uint32_t)1U);
+        int64_t bx3 = scrut.snd;
+        uint64_t rb = a02 & (uint64_t)1U << (uint32_t)(sh - (int64_t)1);
         uint64_t sb = (a02 & mask) ^ rb;
         ap[0U] = a02 & ~mask;
         ite1 = MPFR_Add1sp1_mk_state(sh, bx3, rb, sb);
@@ -359,25 +363,25 @@ MPFR_Add1sp1_mpfr_add1sp1(
           uint64_t *ap = a0.mpfr_d;
           uint64_t *bp = b0.mpfr_d;
           uint64_t *cp = c0.mpfr_d;
-          int32_t bx2 = b0.mpfr_exp;
-          uint64_t sb = cp[0U] << (MPFR_Lib_gmp_NUMB_BITS - d);
-          uint64_t a01 = bp[0U] + (cp[0U] >> d);
-          K___uint64_t_uint64_t_int32_t scrut;
+          int64_t bx2 = b0.mpfr_exp;
+          uint64_t sb = cp[0U] << (uint32_t)(MPFR_Lib_gmp_NUMB_BITS - d);
+          uint64_t a01 = bp[0U] + (cp[0U] >> (uint32_t)d);
+          K___uint64_t_uint64_t_int64_t scrut;
           if (a01 < bp[0U])
             scrut =
               (
-                (K___uint64_t_uint64_t_int32_t){
+                (K___uint64_t_uint64_t_int64_t){
                   .fst = sb | (a01 & (uint64_t)1U),
                   .snd = (uint64_t)0x8000000000000000U | a01 >> (uint32_t)1U,
-                  .thd = bx2 + (int32_t)1
+                  .thd = bx2 + (int64_t)1
                 }
               );
           else
-            scrut = ((K___uint64_t_uint64_t_int32_t){ .fst = sb, .snd = a01, .thd = bx2 });
+            scrut = ((K___uint64_t_uint64_t_int64_t){ .fst = sb, .snd = a01, .thd = bx2 });
           uint64_t sb1 = scrut.fst;
           uint64_t a02 = scrut.snd;
-          int32_t bx3 = scrut.thd;
-          uint64_t rb = a02 & (uint64_t)1U << (sh - (uint32_t)1U);
+          int64_t bx3 = scrut.thd;
+          uint64_t rb = a02 & (uint64_t)1U << (uint32_t)(sh - (int64_t)1);
           uint64_t sb2 = sb1 | ((a02 & mask) ^ rb);
           ap[0U] = a02 & ~mask;
           ite = MPFR_Add1sp1_mk_state(sh, bx3, rb, sb2);
@@ -386,7 +390,7 @@ MPFR_Add1sp1_mpfr_add1sp1(
         {
           uint64_t *ap = a0.mpfr_d;
           uint64_t *bp = b0.mpfr_d;
-          int32_t bx2 = b0.mpfr_exp;
+          int64_t bx2 = b0.mpfr_exp;
           ap[0U] = bp[0U];
           uint64_t rb = (uint64_t)0U;
           uint64_t sb = (uint64_t)1U;
@@ -398,32 +402,32 @@ MPFR_Add1sp1_mpfr_add1sp1(
     }
     else
     {
-      int32_t bx1 = c0.mpfr_exp;
-      int32_t cx1 = b0.mpfr_exp;
-      uint32_t d = (uint32_t)(bx1 - cx1);
-      uint64_t mask = ((uint64_t)1U << sh) - (uint64_t)1U;
+      int64_t bx1 = c0.mpfr_exp;
+      int64_t cx1 = b0.mpfr_exp;
+      int64_t d = bx1 - cx1;
+      uint64_t mask = ((uint64_t)1U << (uint32_t)sh) - (uint64_t)1U;
       MPFR_Add1sp1_state ite1;
       if (d < sh)
       {
         uint64_t *ap = a0.mpfr_d;
         uint64_t *bp = c0.mpfr_d;
         uint64_t *cp = b0.mpfr_d;
-        int32_t bx2 = c0.mpfr_exp;
-        uint64_t a01 = bp[0U] + (cp[0U] >> d);
-        K___uint64_t_int32_t scrut;
+        int64_t bx2 = c0.mpfr_exp;
+        uint64_t a01 = bp[0U] + (cp[0U] >> (uint32_t)d);
+        K___uint64_t_int64_t scrut;
         if (a01 < bp[0U])
           scrut =
             (
-              (K___uint64_t_int32_t){
+              (K___uint64_t_int64_t){
                 .fst = (uint64_t)0x8000000000000000U | a01 >> (uint32_t)1U,
-                .snd = bx2 + (int32_t)1
+                .snd = bx2 + (int64_t)1
               }
             );
         else
-          scrut = ((K___uint64_t_int32_t){ .fst = a01, .snd = bx2 });
+          scrut = ((K___uint64_t_int64_t){ .fst = a01, .snd = bx2 });
         uint64_t a02 = scrut.fst;
-        int32_t bx3 = scrut.snd;
-        uint64_t rb = a02 & (uint64_t)1U << (sh - (uint32_t)1U);
+        int64_t bx3 = scrut.snd;
+        uint64_t rb = a02 & (uint64_t)1U << (uint32_t)(sh - (int64_t)1);
         uint64_t sb = (a02 & mask) ^ rb;
         ap[0U] = a02 & ~mask;
         ite1 = MPFR_Add1sp1_mk_state(sh, bx3, rb, sb);
@@ -436,25 +440,25 @@ MPFR_Add1sp1_mpfr_add1sp1(
           uint64_t *ap = a0.mpfr_d;
           uint64_t *bp = c0.mpfr_d;
           uint64_t *cp = b0.mpfr_d;
-          int32_t bx2 = c0.mpfr_exp;
-          uint64_t sb = cp[0U] << (MPFR_Lib_gmp_NUMB_BITS - d);
-          uint64_t a01 = bp[0U] + (cp[0U] >> d);
-          K___uint64_t_uint64_t_int32_t scrut;
+          int64_t bx2 = c0.mpfr_exp;
+          uint64_t sb = cp[0U] << (uint32_t)(MPFR_Lib_gmp_NUMB_BITS - d);
+          uint64_t a01 = bp[0U] + (cp[0U] >> (uint32_t)d);
+          K___uint64_t_uint64_t_int64_t scrut;
           if (a01 < bp[0U])
             scrut =
               (
-                (K___uint64_t_uint64_t_int32_t){
+                (K___uint64_t_uint64_t_int64_t){
                   .fst = sb | (a01 & (uint64_t)1U),
                   .snd = (uint64_t)0x8000000000000000U | a01 >> (uint32_t)1U,
-                  .thd = bx2 + (int32_t)1
+                  .thd = bx2 + (int64_t)1
                 }
               );
           else
-            scrut = ((K___uint64_t_uint64_t_int32_t){ .fst = sb, .snd = a01, .thd = bx2 });
+            scrut = ((K___uint64_t_uint64_t_int64_t){ .fst = sb, .snd = a01, .thd = bx2 });
           uint64_t sb1 = scrut.fst;
           uint64_t a02 = scrut.snd;
-          int32_t bx3 = scrut.thd;
-          uint64_t rb = a02 & (uint64_t)1U << (sh - (uint32_t)1U);
+          int64_t bx3 = scrut.thd;
+          uint64_t rb = a02 & (uint64_t)1U << (uint32_t)(sh - (int64_t)1);
           uint64_t sb2 = sb1 | ((a02 & mask) ^ rb);
           ap[0U] = a02 & ~mask;
           ite = MPFR_Add1sp1_mk_state(sh, bx3, rb, sb2);
@@ -463,7 +467,7 @@ MPFR_Add1sp1_mpfr_add1sp1(
         {
           uint64_t *ap = a0.mpfr_d;
           uint64_t *bp = c0.mpfr_d;
-          int32_t bx2 = c0.mpfr_exp;
+          int64_t bx2 = c0.mpfr_exp;
           ap[0U] = bp[0U];
           uint64_t rb = (uint64_t)0U;
           uint64_t sb = (uint64_t)1U;
@@ -484,14 +488,14 @@ MPFR_Add1sp1_mpfr_add1sp1(
   {
     uint64_t *ap = a->mpfr_d;
     uint64_t a01 = ap[0U];
-    MPFR_Lib_mpfr_struct uu___62_3483 = a[0U];
+    MPFR_Lib_mpfr_struct uu___72_3478 = a[0U];
     a[0U] =
       (
         (MPFR_Lib_mpfr_struct){
-          .mpfr_prec = uu___62_3483.mpfr_prec,
-          .mpfr_sign = uu___62_3483.mpfr_sign,
+          .mpfr_prec = uu___72_3478.mpfr_prec,
+          .mpfr_sign = uu___72_3478.mpfr_sign,
           .mpfr_exp = st.bx,
-          .mpfr_d = uu___62_3483.mpfr_d
+          .mpfr_d = uu___72_3478.mpfr_d
         }
       );
     if (st.rb == (uint64_t)0U && st.sb == (uint64_t)0U)
@@ -501,7 +505,7 @@ MPFR_Add1sp1_mpfr_add1sp1(
       (
         st.rb
         == (uint64_t)0U
-        || (st.sb == (uint64_t)0U && (a01 & (uint64_t)1U << st.sh) == (uint64_t)0U)
+        || (st.sb == (uint64_t)0U && (a01 & (uint64_t)1U << (uint32_t)st.sh) == (uint64_t)0U)
       )
       {
         int32_t ite;
@@ -514,20 +518,20 @@ MPFR_Add1sp1_mpfr_add1sp1(
       else
       {
         uint64_t *ap1 = a->mpfr_d;
-        ap1[0U] = ap1[0U] + ((uint64_t)1U << st.sh);
+        ap1[0U] = ap1[0U] + ((uint64_t)1U << (uint32_t)st.sh);
         if (ap1[0U] == (uint64_t)0U)
         {
           ap1[0U] = (uint64_t)0x8000000000000000U;
-          if (st.bx + (int32_t)1 <= MPFR_Lib_mpfr_EMAX)
+          if (st.bx + (int64_t)1 <= MPFR_Lib_mpfr_EMAX)
           {
-            MPFR_Lib_mpfr_struct uu___62_3579 = a[0U];
+            MPFR_Lib_mpfr_struct uu___72_3574 = a[0U];
             a[0U] =
               (
                 (MPFR_Lib_mpfr_struct){
-                  .mpfr_prec = uu___62_3579.mpfr_prec,
-                  .mpfr_sign = uu___62_3579.mpfr_sign,
-                  .mpfr_exp = st.bx + (int32_t)1,
-                  .mpfr_d = uu___62_3579.mpfr_d
+                  .mpfr_prec = uu___72_3574.mpfr_prec,
+                  .mpfr_sign = uu___72_3574.mpfr_sign,
+                  .mpfr_exp = st.bx + (int64_t)1,
+                  .mpfr_d = uu___72_3574.mpfr_d
                 }
               );
             return MPFR_Lib_mpfr_RET(a->mpfr_sign);
@@ -553,20 +557,20 @@ MPFR_Add1sp1_mpfr_add1sp1(
     else
     {
       uint64_t *ap1 = a->mpfr_d;
-      ap1[0U] = ap1[0U] + ((uint64_t)1U << st.sh);
+      ap1[0U] = ap1[0U] + ((uint64_t)1U << (uint32_t)st.sh);
       if (ap1[0U] == (uint64_t)0U)
       {
         ap1[0U] = (uint64_t)0x8000000000000000U;
-        if (st.bx + (int32_t)1 <= MPFR_Lib_mpfr_EMAX)
+        if (st.bx + (int64_t)1 <= MPFR_Lib_mpfr_EMAX)
         {
-          MPFR_Lib_mpfr_struct uu___62_3786 = a[0U];
+          MPFR_Lib_mpfr_struct uu___72_3781 = a[0U];
           a[0U] =
             (
               (MPFR_Lib_mpfr_struct){
-                .mpfr_prec = uu___62_3786.mpfr_prec,
-                .mpfr_sign = uu___62_3786.mpfr_sign,
-                .mpfr_exp = st.bx + (int32_t)1,
-                .mpfr_d = uu___62_3786.mpfr_d
+                .mpfr_prec = uu___72_3781.mpfr_prec,
+                .mpfr_sign = uu___72_3781.mpfr_sign,
+                .mpfr_exp = st.bx + (int64_t)1,
+                .mpfr_d = uu___72_3781.mpfr_d
               }
             );
           return MPFR_Lib_mpfr_RET(a->mpfr_sign);
@@ -602,13 +606,13 @@ static K___uint64_t_uint64_t MPFR_Umul_ppmm_umul_ppmm(uint64_t m, uint64_t n1)
     );
 }
 
-typedef struct K___int32_t_uint64_t_uint64_t_s
+typedef struct K___int64_t_uint64_t_uint64_t_s
 {
-  int32_t fst;
+  int64_t fst;
   uint64_t snd;
   uint64_t thd;
 }
-K___int32_t_uint64_t_uint64_t;
+K___int64_t_uint64_t_uint64_t;
 
 static int32_t
 MPFR_Mul_1_mpfr_mul_1(
@@ -616,7 +620,7 @@ MPFR_Mul_1_mpfr_mul_1(
   MPFR_Lib_mpfr_struct *b,
   MPFR_Lib_mpfr_struct *c,
   MPFR_RoundingMode_mpfr_rnd_t rnd_mode,
-  uint32_t p
+  int64_t p
 )
 {
   uint64_t *ap = a->mpfr_d;
@@ -624,38 +628,38 @@ MPFR_Mul_1_mpfr_mul_1(
   uint64_t *cp = c->mpfr_d;
   uint64_t b0 = bp[0U];
   uint64_t c0 = cp[0U];
-  uint32_t sh = MPFR_Lib_gmp_NUMB_BITS - p;
-  uint64_t mask = ((uint64_t)1U << sh) - (uint64_t)1U;
-  int32_t ax = b->mpfr_exp + c->mpfr_exp;
+  int64_t sh = MPFR_Lib_gmp_NUMB_BITS - p;
+  uint64_t mask = ((uint64_t)1U << (uint32_t)sh) - (uint64_t)1U;
+  int64_t ax = b->mpfr_exp + c->mpfr_exp;
   K___uint64_t_uint64_t scrut0 = MPFR_Umul_ppmm_umul_ppmm(b0, c0);
   uint64_t a0 = scrut0.fst;
   uint64_t sb = scrut0.snd;
-  K___int32_t_uint64_t_uint64_t scrut;
+  K___int64_t_uint64_t_uint64_t scrut;
   if (a0 < (uint64_t)0x8000000000000000U)
     scrut =
       (
-        (K___int32_t_uint64_t_uint64_t){
-          .fst = ax - (int32_t)1,
-          .snd = a0 << (uint32_t)1U | sb >> (MPFR_Lib_gmp_NUMB_BITS - (uint32_t)1U),
+        (K___int64_t_uint64_t_uint64_t){
+          .fst = ax - (int64_t)1,
+          .snd = a0 << (uint32_t)1U | sb >> (uint32_t)(MPFR_Lib_gmp_NUMB_BITS - (int64_t)1),
           .thd = sb << (uint32_t)1U
         }
       );
   else
-    scrut = ((K___int32_t_uint64_t_uint64_t){ .fst = ax, .snd = a0, .thd = sb });
-  int32_t ax1 = scrut.fst;
+    scrut = ((K___int64_t_uint64_t_uint64_t){ .fst = ax, .snd = a0, .thd = sb });
+  int64_t ax1 = scrut.fst;
   uint64_t a01 = scrut.snd;
   uint64_t sb1 = scrut.thd;
-  uint64_t rb = a01 & (uint64_t)1U << (sh - (uint32_t)1U);
+  uint64_t rb = a01 & (uint64_t)1U << (uint32_t)(sh - (int64_t)1);
   uint64_t sb2 = sb1 | ((a01 & mask) ^ rb);
   ap[0U] = a01 & ~mask;
-  MPFR_Lib_mpfr_struct uu___63_2736 = a[0U];
+  MPFR_Lib_mpfr_struct uu___73_2756 = a[0U];
   a[0U] =
     (
       (MPFR_Lib_mpfr_struct){
-        .mpfr_prec = uu___63_2736.mpfr_prec,
+        .mpfr_prec = uu___73_2756.mpfr_prec,
         .mpfr_sign = b->mpfr_sign * c->mpfr_sign,
-        .mpfr_exp = uu___63_2736.mpfr_exp,
-        .mpfr_d = uu___63_2736.mpfr_d
+        .mpfr_exp = uu___73_2756.mpfr_exp,
+        .mpfr_d = uu___73_2756.mpfr_d
       }
     );
   uint64_t *ap1 = a->mpfr_d;
@@ -668,7 +672,7 @@ MPFR_Mul_1_mpfr_mul_1(
     if
     (
       ax1
-      == MPFR_Lib_mpfr_EMIN - (int32_t)1
+      == MPFR_Lib_mpfr_EMIN - (int64_t)1
       && a02 == ~mask
       &&
         ((MPFR_RoundingMode_uu___is_MPFR_RNDN(rnd_mode) && rb > (uint64_t)0U)
@@ -677,21 +681,25 @@ MPFR_Mul_1_mpfr_mul_1(
     {
       uint64_t *ap2 = a->mpfr_d;
       uint64_t a03 = ap2[0U];
-      MPFR_Lib_mpfr_struct uu___62_2887 = a[0U];
+      MPFR_Lib_mpfr_struct uu___72_2907 = a[0U];
       a[0U] =
         (
           (MPFR_Lib_mpfr_struct){
-            .mpfr_prec = uu___62_2887.mpfr_prec,
-            .mpfr_sign = uu___62_2887.mpfr_sign,
+            .mpfr_prec = uu___72_2907.mpfr_prec,
+            .mpfr_sign = uu___72_2907.mpfr_sign,
             .mpfr_exp = ax1,
-            .mpfr_d = uu___62_2887.mpfr_d
+            .mpfr_d = uu___72_2907.mpfr_d
           }
         );
       if (rb == (uint64_t)0U && sb2 == (uint64_t)0U)
         return MPFR_Lib_mpfr_RET((int32_t)0);
       else if (MPFR_RoundingMode_uu___is_MPFR_RNDN(rnd_mode))
         if
-        (rb == (uint64_t)0U || (sb2 == (uint64_t)0U && (a03 & (uint64_t)1U << sh) == (uint64_t)0U))
+        (
+          rb
+          == (uint64_t)0U
+          || (sb2 == (uint64_t)0U && (a03 & (uint64_t)1U << (uint32_t)sh) == (uint64_t)0U)
+        )
         {
           int32_t ite;
           if (a->mpfr_sign == (int32_t)1)
@@ -703,22 +711,22 @@ MPFR_Mul_1_mpfr_mul_1(
         else
         {
           uint64_t *ap3 = a->mpfr_d;
-          ap3[0U] = ap3[0U] + ((uint64_t)1U << sh);
+          ap3[0U] = ap3[0U] + ((uint64_t)1U << (uint32_t)sh);
           if (ap3[0U] == (uint64_t)0U)
           {
             ap3[0U] = (uint64_t)0x8000000000000000U;
-            if (ax1 + (int32_t)1 > MPFR_Lib_mpfr_EMAX)
+            if (ax1 + (int64_t)1 > MPFR_Lib_mpfr_EMAX)
               return MPFR_Exceptions_mpfr_overflow(a, rnd_mode, a->mpfr_sign);
             else
             {
-              MPFR_Lib_mpfr_struct uu___62_3027 = a[0U];
+              MPFR_Lib_mpfr_struct uu___72_3047 = a[0U];
               a[0U] =
                 (
                   (MPFR_Lib_mpfr_struct){
-                    .mpfr_prec = uu___62_3027.mpfr_prec,
-                    .mpfr_sign = uu___62_3027.mpfr_sign,
-                    .mpfr_exp = ax1 + (int32_t)1,
-                    .mpfr_d = uu___62_3027.mpfr_d
+                    .mpfr_prec = uu___72_3047.mpfr_prec,
+                    .mpfr_sign = uu___72_3047.mpfr_sign,
+                    .mpfr_exp = ax1 + (int64_t)1,
+                    .mpfr_d = uu___72_3047.mpfr_d
                   }
                 );
               return MPFR_Lib_mpfr_RET(a->mpfr_sign);
@@ -739,22 +747,22 @@ MPFR_Mul_1_mpfr_mul_1(
       else
       {
         uint64_t *ap3 = a->mpfr_d;
-        ap3[0U] = ap3[0U] + ((uint64_t)1U << sh);
+        ap3[0U] = ap3[0U] + ((uint64_t)1U << (uint32_t)sh);
         if (ap3[0U] == (uint64_t)0U)
         {
           ap3[0U] = (uint64_t)0x8000000000000000U;
-          if (ax1 + (int32_t)1 > MPFR_Lib_mpfr_EMAX)
+          if (ax1 + (int64_t)1 > MPFR_Lib_mpfr_EMAX)
             return MPFR_Exceptions_mpfr_overflow(a, rnd_mode, a->mpfr_sign);
           else
           {
-            MPFR_Lib_mpfr_struct uu___62_3217 = a[0U];
+            MPFR_Lib_mpfr_struct uu___72_3237 = a[0U];
             a[0U] =
               (
                 (MPFR_Lib_mpfr_struct){
-                  .mpfr_prec = uu___62_3217.mpfr_prec,
-                  .mpfr_sign = uu___62_3217.mpfr_sign,
-                  .mpfr_exp = ax1 + (int32_t)1,
-                  .mpfr_d = uu___62_3217.mpfr_d
+                  .mpfr_prec = uu___72_3237.mpfr_prec,
+                  .mpfr_sign = uu___72_3237.mpfr_sign,
+                  .mpfr_exp = ax1 + (int64_t)1,
+                  .mpfr_d = uu___72_3237.mpfr_d
                 }
               );
             return MPFR_Lib_mpfr_RET(a->mpfr_sign);
@@ -769,7 +777,7 @@ MPFR_Mul_1_mpfr_mul_1(
       MPFR_RoundingMode_uu___is_MPFR_RNDN(rnd_mode)
       &&
         (ax1
-        < MPFR_Lib_mpfr_EMIN - (int32_t)1
+        < MPFR_Lib_mpfr_EMIN - (int64_t)1
         || (a02 == (uint64_t)0x8000000000000000U && (rb | sb2) == (uint64_t)0U))
     )
       return MPFR_Exceptions_mpfr_underflow(a, MPFR_RoundingMode_MPFR_RNDZ, a->mpfr_sign);
@@ -780,20 +788,25 @@ MPFR_Mul_1_mpfr_mul_1(
   {
     uint64_t *ap2 = a->mpfr_d;
     uint64_t a03 = ap2[0U];
-    MPFR_Lib_mpfr_struct uu___62_3402 = a[0U];
+    MPFR_Lib_mpfr_struct uu___72_3422 = a[0U];
     a[0U] =
       (
         (MPFR_Lib_mpfr_struct){
-          .mpfr_prec = uu___62_3402.mpfr_prec,
-          .mpfr_sign = uu___62_3402.mpfr_sign,
+          .mpfr_prec = uu___72_3422.mpfr_prec,
+          .mpfr_sign = uu___72_3422.mpfr_sign,
           .mpfr_exp = ax1,
-          .mpfr_d = uu___62_3402.mpfr_d
+          .mpfr_d = uu___72_3422.mpfr_d
         }
       );
     if (rb == (uint64_t)0U && sb2 == (uint64_t)0U)
       return MPFR_Lib_mpfr_RET((int32_t)0);
     else if (MPFR_RoundingMode_uu___is_MPFR_RNDN(rnd_mode))
-      if (rb == (uint64_t)0U || (sb2 == (uint64_t)0U && (a03 & (uint64_t)1U << sh) == (uint64_t)0U))
+      if
+      (
+        rb
+        == (uint64_t)0U
+        || (sb2 == (uint64_t)0U && (a03 & (uint64_t)1U << (uint32_t)sh) == (uint64_t)0U)
+      )
       {
         int32_t ite;
         if (a->mpfr_sign == (int32_t)1)
@@ -805,22 +818,22 @@ MPFR_Mul_1_mpfr_mul_1(
       else
       {
         uint64_t *ap3 = a->mpfr_d;
-        ap3[0U] = ap3[0U] + ((uint64_t)1U << sh);
+        ap3[0U] = ap3[0U] + ((uint64_t)1U << (uint32_t)sh);
         if (ap3[0U] == (uint64_t)0U)
         {
           ap3[0U] = (uint64_t)0x8000000000000000U;
-          if (ax1 + (int32_t)1 > MPFR_Lib_mpfr_EMAX)
+          if (ax1 + (int64_t)1 > MPFR_Lib_mpfr_EMAX)
             return MPFR_Exceptions_mpfr_overflow(a, rnd_mode, a->mpfr_sign);
           else
           {
-            MPFR_Lib_mpfr_struct uu___62_3542 = a[0U];
+            MPFR_Lib_mpfr_struct uu___72_3562 = a[0U];
             a[0U] =
               (
                 (MPFR_Lib_mpfr_struct){
-                  .mpfr_prec = uu___62_3542.mpfr_prec,
-                  .mpfr_sign = uu___62_3542.mpfr_sign,
-                  .mpfr_exp = ax1 + (int32_t)1,
-                  .mpfr_d = uu___62_3542.mpfr_d
+                  .mpfr_prec = uu___72_3562.mpfr_prec,
+                  .mpfr_sign = uu___72_3562.mpfr_sign,
+                  .mpfr_exp = ax1 + (int64_t)1,
+                  .mpfr_d = uu___72_3562.mpfr_d
                 }
               );
             return MPFR_Lib_mpfr_RET(a->mpfr_sign);
@@ -841,22 +854,22 @@ MPFR_Mul_1_mpfr_mul_1(
     else
     {
       uint64_t *ap3 = a->mpfr_d;
-      ap3[0U] = ap3[0U] + ((uint64_t)1U << sh);
+      ap3[0U] = ap3[0U] + ((uint64_t)1U << (uint32_t)sh);
       if (ap3[0U] == (uint64_t)0U)
       {
         ap3[0U] = (uint64_t)0x8000000000000000U;
-        if (ax1 + (int32_t)1 > MPFR_Lib_mpfr_EMAX)
+        if (ax1 + (int64_t)1 > MPFR_Lib_mpfr_EMAX)
           return MPFR_Exceptions_mpfr_overflow(a, rnd_mode, a->mpfr_sign);
         else
         {
-          MPFR_Lib_mpfr_struct uu___62_3732 = a[0U];
+          MPFR_Lib_mpfr_struct uu___72_3752 = a[0U];
           a[0U] =
             (
               (MPFR_Lib_mpfr_struct){
-                .mpfr_prec = uu___62_3732.mpfr_prec,
-                .mpfr_sign = uu___62_3732.mpfr_sign,
-                .mpfr_exp = ax1 + (int32_t)1,
-                .mpfr_d = uu___62_3732.mpfr_d
+                .mpfr_prec = uu___72_3752.mpfr_prec,
+                .mpfr_sign = uu___72_3752.mpfr_sign,
+                .mpfr_exp = ax1 + (int64_t)1,
+                .mpfr_d = uu___72_3752.mpfr_d
               }
             );
           return MPFR_Lib_mpfr_RET(a->mpfr_sign);
@@ -874,7 +887,7 @@ int32_t
   MPFR_Lib_mpfr_struct *x1,
   MPFR_Lib_mpfr_struct *x2,
   MPFR_RoundingMode_mpfr_rnd_t x3,
-  uint32_t x4
+  int64_t x4
 ) = MPFR_Add1sp1_mpfr_add1sp1;
 
 int32_t
@@ -883,6 +896,6 @@ int32_t
   MPFR_Lib_mpfr_struct *x1,
   MPFR_Lib_mpfr_struct *x2,
   MPFR_RoundingMode_mpfr_rnd_t x3,
-  uint32_t x4
+  int64_t x4
 ) = MPFR_Mul_1_mpfr_mul_1;
 
