code/mpfr/test/Test_Add1sp1.ml
@@ -2,24 +2,31 @@ open Prims
 open Printf
 
 type i32 = FStar_Int32.t
-type u32 = FStar_UInt32.t
+type i64 = FStar_Int64.t
 type u64 = FStar_UInt64.t
 
-let (cmod : Prims.int -> Prims.int) =
+let (cmod32 : Prims.int -> Prims.int) =
   fun x  ->
     if x > (Prims.parse_int "2147483647")
     then x - (Prims.parse_int "4294967296")
     else x
-
-let (print_u32 : FStar_UInt32.t -> unit) =
-  fun x  ->
-    FStar_HyperStack_IO.print_string (Prims.string_of_int (FStar_UInt32.v x));
-    FStar_HyperStack_IO.print_string " "
   
 let (print_i32 : FStar_Int32.t -> unit) =
   fun x  ->
     FStar_HyperStack_IO.print_string
-      (Prims.string_of_int (cmod (FStar_Int32.v x)));
+      (Prims.string_of_int (cmod32 (FStar_Int32.v x)));
+    FStar_HyperStack_IO.print_string " "
+
+let (cmod64 : Prims.int -> Prims.int) =
+  fun x  ->
+    if x > (Prims.parse_int "9223372036854775807")
+    then x - (Prims.parse_int "18446744073709551616")
+    else x
+  
+let (print_i64 : FStar_Int64.t -> unit) =
+  fun x  ->
+    FStar_HyperStack_IO.print_string
+      (Prims.string_of_int (cmod64 (FStar_Int64.v x)));
     FStar_HyperStack_IO.print_string " "
   
 let (print_u64 : FStar_UInt64.t -> unit) =
@@ -52,12 +59,12 @@ fun str ->
 	       else MPFR_RoundingMode.MPFR_RNDA) in
     let s    = FStar_Int32.int_to_t   (Prims.parse_int (List.nth tokens 0)) in
     let bp   = FStar_UInt64.uint_to_t (Prims.parse_int (List.nth tokens 1)) in
-    let bx   = FStar_Int32.int_to_t   (Prims.parse_int (List.nth tokens 2)) in
+    let bx   = FStar_Int64.int_to_t   (Prims.parse_int (List.nth tokens 2)) in
     let cp   = FStar_UInt64.uint_to_t (Prims.parse_int (List.nth tokens 4)) in
-    let cx   = FStar_Int32.int_to_t   (Prims.parse_int (List.nth tokens 5)) in
-    let p    = FStar_UInt32.uint_to_t (Prims.parse_int (List.nth tokens 7)) in
+    let cx   = FStar_Int64.int_to_t   (Prims.parse_int (List.nth tokens 5)) in
+    let p    = FStar_Int64.int_to_t  (Prims.parse_int (List.nth tokens 7)) in
     let rp   = FStar_UInt64.uint_to_t (Prims.parse_int (List.nth tokens 9)) in
-    let rx   = FStar_Int32.int_to_t   (Prims.parse_int (List.nth tokens 10)) in
+    let rx   = FStar_Int64.int_to_t   (Prims.parse_int (List.nth tokens 10)) in
     let flag = FStar_Int32.int_to_t   (Prims.parse_int (List.nth tokens 11)) in
     let bm = FStar_Buffer.createL [bp]  in
     let bs = MPFR_Lib.mk_mpfr_struct p s bx bm  in
@@ -76,9 +83,9 @@ fun str ->
     FStar_HyperStack_IO.print_string "Result: \n";
     print_i32 asign;
     print_u64 ap;
-    print_i32 ax;
+    print_i64 ax;
     print_i32 af;
-    if (((FStar_UInt64.eq ap rp) && (FStar_Int32.eq ax rx) || (FStar_Int32.eq ax rx) && (FStar_Int32.eq ax MPFR_Lib.mpfr_EXP_INF)) && (FStar_Int32.eq asign s) && (FStar_Int32.eq af flag)) then
+    if (((FStar_UInt64.eq ap rp) && (FStar_Int64.eq ax rx) || (FStar_Int64.eq ax rx) && (FStar_Int64.eq ax MPFR_Lib.mpfr_EXP_INF)) && (FStar_Int32.eq asign s) && (FStar_Int32.eq af flag)) then
         print_string "YES!!!\n"
     else begin
         raise Exit;
