code/mpfr/MPFR.Add1sp1.Lemma.fst
@@ -15,19 +15,19 @@ open MPFR.Round.Spec
 open MPFR.Dyadic
 open MPFR.Maths
 
-module I64 = FStar.Int64
 module I32 = FStar.Int32
+module I64 = FStar.Int64
 module U32 = FStar.UInt32
 
 #set-options "--z3refresh --z3rlimit 100 --max_fuel 1 --initial_fuel 0 --max_ifuel 1 --initial_ifuel 0"
 
 (* intermediate results *)
-private type mpfr_tmp_exp_t = x:mpfr_exp_t{I32.(x >=^ mpfr_EMIN /\ x <=^ mpfr_EMAX +^ 1l)}
+private type mpfr_tmp_exp_t = x:mpfr_exp_t{I64.(x >=^ mpfr_EMIN /\ x <=^ mpfr_EMAX +^ 1L)}
 
 (* pre/post-condition for mpfr_add1sp1_any *)
 let mpfr_add1sp1_common_pre_cond a b c (p:mpfr_prec_t) h =
     mpfr_reg_cond_ h b /\ mpfr_reg_cond_ h c /\
-    0 < U32.v p /\ U32.v p < U32.v gmp_NUMB_BITS /\
+    0 < I64.v p /\ I64.v p < I64.v gmp_NUMB_BITS /\
     a.mpfr_prec = p /\ b.mpfr_prec = p /\ c.mpfr_prec = p /\
     live h a.mpfr_d /\ live h b.mpfr_d /\ live h c.mpfr_d /\
     length a.mpfr_d = 1 /\ length b.mpfr_d = 1 /\ length c.mpfr_d = 1
@@ -38,27 +38,27 @@ let mpfr_add1sp1_any_pre_cond a b c (p:mpfr_prec_t) h =
     
 (* pre-condition for mpfr_add1sp1_gt where b.exp > c.exp *)
 let mpfr_add1sp1_gt_pre_cond a b c sh h =
-    I32.v b.mpfr_exp > I32.v c.mpfr_exp /\
-    U32.v sh = U32.v gmp_NUMB_BITS - U32.v a.mpfr_prec /\
-    mpfr_add1sp1_common_pre_cond a b c U32.(gmp_NUMB_BITS -^ sh) h
+    I64.v b.mpfr_exp > I64.v c.mpfr_exp /\
+    I64.v sh = I64.v gmp_NUMB_BITS - I64.v a.mpfr_prec /\
+    mpfr_add1sp1_common_pre_cond a b c I64.(gmp_NUMB_BITS -^ sh) h
 
 (* lemmas and implementation for mpfr_add1sp1_gt_branch1 where d < sh *)
 let mpfr_add1sp1_gt_branch1_pre_cond a b c sh d mask h =
     mpfr_add1sp1_gt_pre_cond a b c sh h /\
-    U32.v d = I32.v b.mpfr_exp - I32.v c.mpfr_exp /\
-    v mask = pow2 (U32.v sh) - 1 /\
-    U32.v d < U32.v sh
+    I64.v d = I64.v b.mpfr_exp - I64.v c.mpfr_exp /\
+    v mask = pow2 (I64.v sh) - 1 /\
+    I64.v d < I64.v sh
     
 (* lemmas and implementation for mpfr_add1sp1_gt_branch1 where sh <= d < 64 *)
 let mpfr_add1sp1_gt_branch2_pre_cond a b c sh d mask h =
     mpfr_add1sp1_gt_pre_cond a b c sh h /\
-    U32.v d = I32.v b.mpfr_exp - I32.v c.mpfr_exp /\
-    v mask = pow2 (U32.v sh) - 1 /\
-    U32.v d >= U32.v sh /\ U32.v d < U32.v gmp_NUMB_BITS
+    I64.v d = I64.v b.mpfr_exp - I64.v c.mpfr_exp /\
+    v mask = pow2 (I64.v sh) - 1 /\
+    I64.v d >= I64.v sh /\ I64.v d < I64.v gmp_NUMB_BITS
     
 val mpfr_add1sp1_gt_branch12_a0_bx_lemma:
     h:mem -> a:mpfr_struct -> b:mpfr_struct -> c:mpfr_struct ->
-    sh:mpfr_reg_prec_t -> d:u32 -> mask:mp_limb_t -> Lemma
+    sh:mpfr_reg_prec_t -> d:i64 -> mask:mp_limb_t -> Lemma
     (requires (mpfr_add1sp1_gt_branch1_pre_cond a b c sh d mask h \/
                mpfr_add1sp1_gt_branch2_pre_cond a b c sh d mask h))
     (ensures  (
@@ -66,17 +66,17 @@ val mpfr_add1sp1_gt_branch12_a0_bx_lemma:
     let bx = b.mpfr_exp in
     let b0 = Seq.index (as_seq h b.mpfr_d) 0 in
     let c0 = Seq.index (as_seq h c.mpfr_d) 0 in
-    let a0 = b0 +%^ (c0 >>^ d) in
-    let a0, bx = if a0 <^ b0 then mpfr_LIMB_HIGHBIT |^ (a0 >>^ 1ul), I32.(bx +^ 1l) else a0, bx in
-    v a0 = r.limb / pow2 (r.len - 64) /\ I32.v bx = r.exp))
+    let a0 = b0 +%^ (c0 >>^ (int64_to_uint32) d) in
+    let a0, bx = if a0 <^ b0 then mpfr_LIMB_HIGHBIT |^ (a0 >>^ 1ul), I64.(bx +^ 1L) else a0, bx in
+    v a0 = r.limb / pow2 (r.len - 64) /\ I64.v bx = r.exp))
 
 let mpfr_add1sp1_gt_branch12_a0_bx_lemma h a b c sh d mask =
     let r = add1sp_exact (as_reg_fp_ h b) (as_reg_fp_ h c) in
     let bx = b.mpfr_exp in
     let b0 = Seq.index (as_seq h b.mpfr_d) 0 in
     let c0 = Seq.index (as_seq h c.mpfr_d) 0 in
-    let a0 = b0 +%^ (c0 >>^ d) in
-    let t0 = v b0 + v c0 / pow2 (U32.v d) in
+    let a0 = b0 +%^ (c0 >>^ (int64_to_uint32 d)) in
+    let t0 = v b0 + v c0 / pow2 (I64.v d) in
     //! assert(v a0 = t0 % pow2 64);
     let a0, bx =
         if a0 <^ b0 then begin
@@ -84,7 +84,7 @@ let mpfr_add1sp1_gt_branch12_a0_bx_lemma h a b c sh d mask =
 	    lemma_add_div (v a0) (pow2 63) 2;
 	    //! assert(pow2 63 + v a0 / 2 = t0 / pow2 1);
 	    let a0' = mpfr_LIMB_HIGHBIT |^ (a0 >>^ 1ul) in
-	    let bx' = I32.(bx +^ 1l) in
+	    let bx' = I64.(bx +^ 1L) in
 	    lemma_logor_pow2_disjoint mpfr_LIMB_HIGHBIT (a0 >>^ 1ul) 63;
 	    //! assert(v a0' = t0 / pow2 1);
 	    a0', bx'
@@ -92,23 +92,23 @@ let mpfr_add1sp1_gt_branch12_a0_bx_lemma h a b c sh d mask =
 	    //! assert(v a0 = t0 / pow2 0);
 	    a0, bx
 	end in
-    //! assert(v a0 = t0 / pow2 (I32.v bx - I32.v b.mpfr_exp));
-    lemma_add_div (v c0) (v b0) (pow2 (U32.v d));
-    //! assert(t0 = r.limb / pow2 (U32.v d));
-    lemma_pow2_div_div r.limb (U32.v d) (I32.v bx - I32.v b.mpfr_exp);
-    //! assert(v a0 = r.limb / pow2 (I32.v bx - I32.v b.mpfr_exp + U32.v d));
-    lemma_pow2_div_range r.limb (I32.v bx - I32.v b.mpfr_exp + U32.v d) r.len;
-    lemma_bit_length (v a0) 64 (r.len - I32.v bx + I32.v b.mpfr_exp - U32.v d);
-    assert(I32.v bx = r.len + I32.v b.mpfr_exp - U32.v d - 64);
+    //! assert(v a0 = t0 / pow2 (I64.v bx - I64.v b.mpfr_exp));
+    lemma_add_div (v c0) (v b0) (pow2 (I64.v d));
+    //! assert(t0 = r.limb / pow2 (I64.v d));
+    lemma_pow2_div_div r.limb (I64.v d) (I64.v bx - I64.v b.mpfr_exp);
+    //! assert(v a0 = r.limb / pow2 (I64.v bx - I64.v b.mpfr_exp + I64.v d));
+    lemma_pow2_div_range r.limb (I64.v bx - I64.v b.mpfr_exp + I64.v d) r.len;
+    lemma_bit_length (v a0) 64 (r.len - I64.v bx + I64.v b.mpfr_exp - I64.v d);
+    assert(I64.v bx = r.len + I64.v b.mpfr_exp - I64.v d - 64);
     ()
 
 val mpfr_add1sp1_gt_branch12_value_lemma:
     h:mem -> a:mpfr_struct -> b:mpfr_struct -> c:mpfr_struct ->
-    sh:mpfr_reg_prec_t -> d:u32 -> mask:mp_limb_t -> Lemma
+    sh:mpfr_reg_prec_t -> d:i64 -> mask:mp_limb_t -> Lemma
     (requires (mpfr_add1sp1_gt_branch1_pre_cond a b c sh d mask h \/
                mpfr_add1sp1_gt_branch2_pre_cond a b c sh d mask h))
     (ensures  (
-    let p = U32.v a.mpfr_prec in
+    let p = I64.v a.mpfr_prec in
     let r = add1sp_exact (as_reg_fp_ h b) (as_reg_fp_ h c) in
     let r = high_mant r p in
     let bp = b.mpfr_d in
@@ -116,23 +116,23 @@ val mpfr_add1sp1_gt_branch12_value_lemma:
     let bx = b.mpfr_exp in
     let b0 = Seq.index (as_seq h bp) 0 in
     let c0 = Seq.index (as_seq h cp) 0 in
-    let a0 = b0 +%^ (c0 >>^ d) in
-    let a0, bx = if a0 <^ b0 then mpfr_LIMB_HIGHBIT |^ (a0 >>^ 1ul), I32.(bx +^ 1l) else a0, bx in
+    let a0 = b0 +%^ (c0 >>^ (int64_to_uint32 d)) in
+    let a0, bx = if a0 <^ b0 then mpfr_LIMB_HIGHBIT |^ (a0 >>^ 1ul), I64.(bx +^ 1L) else a0, bx in
     let a0 = a0 &^ (lognot mask) in
-    v a0 * pow2 (r.len - 64) = r.limb /\ I32.v bx = r.exp /\
+    v a0 * pow2 (r.len - 64) = r.limb /\ I64.v bx = r.exp /\
     v a0 >= pow2 63 /\ v a0 % pow2 (64 - p) = 0))
 
 let mpfr_add1sp1_gt_branch12_value_lemma h a b c sh d mask =
-    let p = U32.v a.mpfr_prec in
+    let p = I64.v a.mpfr_prec in
     let r = add1sp_exact (as_reg_fp_ h b) (as_reg_fp_ h c) in
     let bp = b.mpfr_d in
     let cp = c.mpfr_d in
     let bx = b.mpfr_exp in
     let b0 = Seq.index (as_seq h bp) 0 in
     let c0 = Seq.index (as_seq h cp) 0 in
-    let a0 = b0 +%^ (c0 >>^ d) in
-    let t0 = v b0 + v c0 / pow2 (U32.v d) in
-    let a0, bx = if a0 <^ b0 then mpfr_LIMB_HIGHBIT |^ (a0 >>^ 1ul), I32.(bx +^ 1l) else a0, bx in
+    let a0 = b0 +%^ (c0 >>^ (int64_to_uint32 d)) in
+    let t0 = v b0 + v c0 / pow2 (I64.v d) in
+    let a0, bx = if a0 <^ b0 then mpfr_LIMB_HIGHBIT |^ (a0 >>^ 1ul), I64.(bx +^ 1L) else a0, bx in
     mpfr_add1sp1_gt_branch12_a0_bx_lemma h a b c sh d mask;
     lemma_pow2_div_div (r.limb) (r.len - 64) (64 - p);
     //! assert(v a0 / pow2 (64 - p) = r.limb / pow2 (r.len - p));
@@ -152,116 +152,116 @@ let mpfr_add1sp1_gt_branch12_value_lemma h a b c sh d mask =
 
 val mpfr_add1sp1_gt_branch12_rb_lemma:
     h:mem -> a:mpfr_struct -> b:mpfr_struct -> c:mpfr_struct ->
-    sh:mpfr_reg_prec_t -> d:u32 -> mask:mp_limb_t -> Lemma
+    sh:mpfr_reg_prec_t -> d:i64 -> mask:mp_limb_t -> Lemma
     (requires (mpfr_add1sp1_gt_branch1_pre_cond a b c sh d mask h \/
                mpfr_add1sp1_gt_branch2_pre_cond a b c sh d mask h))
     (ensures  (
-    let p = U32.v a.mpfr_prec in
+    let p = I64.v a.mpfr_prec in
     let r = add1sp_exact (as_reg_fp_ h b) (as_reg_fp_ h c) in
     let bp = b.mpfr_d in
     let cp = c.mpfr_d in
     let b0 = Seq.index (as_seq h bp) 0 in
     let c0 = Seq.index (as_seq h cp) 0 in
-    let a0 = b0 +%^ (c0 >>^ d) in
+    let a0 = b0 +%^ (c0 >>^ (int64_to_uint32 d)) in
     let a0 = if a0 <^ b0 then mpfr_LIMB_HIGHBIT |^ (a0 >>^ 1ul) else a0 in
-    let rb = a0 &^ (mpfr_LIMB_ONE <<^ U32.(sh -^ 1ul)) in
+    let rb = a0 &^ (mpfr_LIMB_ONE <<^ (int64_to_uint32 I64.(sh -^ 1L))) in
     rb_def r p = (v rb <> 0)))
 
 let mpfr_add1sp1_gt_branch12_rb_lemma h a b c sh d mask = 
-    let p = U32.v a.mpfr_prec in
+    let p = I64.v a.mpfr_prec in
     let r = add1sp_exact (as_reg_fp_ h b) (as_reg_fp_ h c) in
     let bp = b.mpfr_d in
     let cp = c.mpfr_d in
     let b0 = Seq.index (as_seq h bp) 0 in
     let c0 = Seq.index (as_seq h cp) 0 in
-    let a0 = b0 +%^ (c0 >>^ d) in
+    let a0 = b0 +%^ (c0 >>^ (int64_to_uint32 d)) in
     let a0 = if a0 <^ b0 then mpfr_LIMB_HIGHBIT |^ (a0 >>^ 1ul) else a0 in
     mpfr_add1sp1_gt_branch12_a0_bx_lemma h a b c sh d mask;
     //! assert(v a0 = r.limb / pow2 (r.len - 64));
     UInt.slice_left_lemma (UInt.to_vec #r.len r.limb) 64;
     //! assert(UInt.nth (v a0) p = UInt.nth #r.len r.limb p);
-    let rb = a0 &^ (mpfr_LIMB_ONE <<^ U32.(sh -^ 1ul)) in
-    lemma_pow2_small_mod (U32.v sh - 1) 64;
-    //! assert(v (mpfr_LIMB_ONE <<^ U32.(sh -^ 1ul)) = pow2 (U32.v sh - 1));
-    lemma_bit_mask_value a0 (mpfr_LIMB_ONE <<^ U32.(sh -^ 1ul)) p
+    let rb = a0 &^ (mpfr_LIMB_ONE <<^ (int64_to_uint32 I64.(sh -^ 1L))) in
+    lemma_pow2_small_mod (I64.v sh - 1) 64;
+    //! assert(v (mpfr_LIMB_ONE <<^ I64.(sh -^ 1ul)) = pow2 (I64.v sh - 1));
+    lemma_bit_mask_value a0 (mpfr_LIMB_ONE <<^ (int64_to_uint32 I64.(sh -^ 1L))) p
 
 val mpfr_add1sp1_gt_branch12_former_sb_lemma:
     h:mem -> a:mpfr_struct -> b:mpfr_struct -> c:mpfr_struct ->
-    sh:mpfr_reg_prec_t -> d:u32 -> mask:mp_limb_t -> Lemma
+    sh:mpfr_reg_prec_t -> d:i64 -> mask:mp_limb_t -> Lemma
     (requires (mpfr_add1sp1_gt_branch1_pre_cond a b c sh d mask h \/
                mpfr_add1sp1_gt_branch2_pre_cond a b c sh d mask h))
     (ensures  (
-    let p = U32.v a.mpfr_prec in
+    let p = I64.v a.mpfr_prec in
     let r = add1sp_exact (as_reg_fp_ h b) (as_reg_fp_ h c) in
     let bp = b.mpfr_d in
     let cp = c.mpfr_d in
     let b0 = Seq.index (as_seq h bp) 0 in
     let c0 = Seq.index (as_seq h cp) 0 in
-    let a0 = b0 +%^ (c0 >>^ d) in
+    let a0 = b0 +%^ (c0 >>^ (int64_to_uint32 d)) in
     let a0 = if a0 <^ b0 then mpfr_LIMB_HIGHBIT |^ (a0 >>^ 1ul) else a0 in
-    let rb = a0 &^ (mpfr_LIMB_ONE <<^ U32.(sh -^ 1ul)) in
+    let rb = a0 &^ (mpfr_LIMB_ONE <<^ (int64_to_uint32 I64.(sh -^ 1L))) in
     let sb = (a0 &^ mask) ^^ rb in
     v sb = r.limb % pow2 (r.len - p - 1) / pow2 (r.len - 64)))
 
 let mpfr_add1sp1_gt_branch12_former_sb_lemma h a b c sh d mask =
-    let p = U32.v a.mpfr_prec in
+    let p = I64.v a.mpfr_prec in
     let r = add1sp_exact (as_reg_fp_ h b) (as_reg_fp_ h c) in
     let bp = b.mpfr_d in
     let cp = c.mpfr_d in
     let b0 = Seq.index (as_seq h bp) 0 in
     let c0 = Seq.index (as_seq h cp) 0 in
-    let a0 = b0 +%^ (c0 >>^ d) in
+    let a0 = b0 +%^ (c0 >>^ (int64_to_uint32 d)) in
     let a0 = if a0 <^ b0 then mpfr_LIMB_HIGHBIT |^ (a0 >>^ 1ul) else a0 in
-    let rb = a0 &^ (mpfr_LIMB_ONE <<^ U32.(sh -^ 1ul)) in
+    let rb = a0 &^ (mpfr_LIMB_ONE <<^ (int64_to_uint32 I64.(sh -^ 1L))) in
     let sb = (a0 &^ mask) ^^ rb in
-    lemma_pow2_small_mod (U32.v sh - 1) 64;
-    //! assert(v (mpfr_LIMB_ONE <<^ U32.(sh -^ 1ul)) = pow2 (U32.v sh - 1));
-    lemma_bit_mask (mpfr_LIMB_ONE <<^ U32.(sh -^ 1ul)) (64 - U32.v sh);
-    lemma_tail_mask mask (U32.v sh);
-    let rmask = mpfr_LIMB_MASK U32.(sh -^ 1ul) in
-    UInt.nth_lemma #64 (v (mask ^^ (mpfr_LIMB_ONE <<^ U32.(sh -^ 1ul)))) (v rmask);
-    lemma_xor_and_distr (v a0) (v mask) (v (mpfr_LIMB_ONE <<^ U32.(sh -^ 1ul)));
+    lemma_pow2_small_mod (I64.v sh - 1) 64;
+    //! assert(v (mpfr_LIMB_ONE <<^ I64.(sh -^ 1ul)) = pow2 (I64.v sh - 1));
+    lemma_bit_mask (mpfr_LIMB_ONE <<^ (int64_to_uint32 I64.(sh -^ 1L))) (64 - I64.v sh);
+    lemma_tail_mask mask (I64.v sh);
+    let rmask = mpfr_LIMB_MASK (int64_to_uint32 I64.(sh -^ 1L)) in
+    UInt.nth_lemma #64 (v (mask ^^ (mpfr_LIMB_ONE <<^ (int64_to_uint32 I64.(sh -^ 1L))))) (v rmask);
+    lemma_xor_and_distr (v a0) (v mask) (v (mpfr_LIMB_ONE <<^ (int64_to_uint32 I64.(sh -^ 1L))));
     //! assert(sb = (a0 &^ rmask));
-    lemma_tail_mask_value a0 rmask (U32.v sh - 1);
-    //! assert(v sb = (v a0) % pow2 (U32.v sh - 1));
+    lemma_tail_mask_value a0 rmask (I64.v sh - 1);
+    //! assert(v sb = (v a0) % pow2 (I64.v sh - 1));
     mpfr_add1sp1_gt_branch12_a0_bx_lemma h a b c sh d mask;
     lemma_pow2_mod_div r.limb (r.len - p - 1) (r.len - 64)
 
 val mpfr_add1sp1_gt_branch1_sb_lemma:
     h:mem -> a:mpfr_struct -> b:mpfr_struct -> c:mpfr_struct ->
-    sh:mpfr_reg_prec_t -> d:u32 -> mask:mp_limb_t -> Lemma
+    sh:mpfr_reg_prec_t -> d:i64 -> mask:mp_limb_t -> Lemma
     (requires (mpfr_add1sp1_gt_branch1_pre_cond a b c sh d mask h))
     (ensures  (
-    let p = U32.v a.mpfr_prec in
+    let p = I64.v a.mpfr_prec in
     let r = add1sp_exact (as_reg_fp_ h b) (as_reg_fp_ h c) in
     let bp = b.mpfr_d in
     let cp = c.mpfr_d in
     let b0 = Seq.index (as_seq h bp) 0 in
     let c0 = Seq.index (as_seq h cp) 0 in
-    let a0 = b0 +%^ (c0 >>^ d) in
+    let a0 = b0 +%^ (c0 >>^ (int64_to_uint32 d)) in
     let a0 = if a0 <^ b0 then mpfr_LIMB_HIGHBIT |^ (a0 >>^ 1ul) else a0 in
-    let rb = a0 &^ (mpfr_LIMB_ONE <<^ U32.(sh -^ 1ul)) in
+    let rb = a0 &^ (mpfr_LIMB_ONE <<^ (int64_to_uint32 I64.(sh -^ 1L))) in
     let sb = (a0 &^ mask) ^^ rb in
     sb_def r p = (v sb <> 0)))
 
 let mpfr_add1sp1_gt_branch1_sb_lemma h a b c sh d mask =
-    let p = U32.v a.mpfr_prec in
+    let p = I64.v a.mpfr_prec in
     let r = add1sp_exact (as_reg_fp_ h b) (as_reg_fp_ h c) in
     let bp = b.mpfr_d in
     let cp = c.mpfr_d in
     let b0 = Seq.index (as_seq h bp) 0 in
     let c0 = Seq.index (as_seq h cp) 0 in
-    let a0 = b0 +%^ (c0 >>^ d) in
+    let a0 = b0 +%^ (c0 >>^ (int64_to_uint32 d)) in
     let a0 = if a0 <^ b0 then mpfr_LIMB_HIGHBIT |^ (a0 >>^ 1ul) else a0 in
-    let rb = a0 &^ (mpfr_LIMB_ONE <<^ U32.(sh -^ 1ul)) in
+    let rb = a0 &^ (mpfr_LIMB_ONE <<^ (int64_to_uint32 I64.(sh -^ 1L))) in
     let sb = (a0 &^ mask) ^^ rb in
     mpfr_add1sp1_gt_branch12_a0_bx_lemma h a b c sh d mask;
-    lemma_pow2_mul_mod (v b0) (U32.v d) (r.len - 64);
-    lemma_pow2_mod_mod_zero (v b0) (U32.v sh) (r.len - 64 - U32.v d);
-    //! assert(v b0 * pow2 (U32.v d) % pow2 (r.len - 64) = 0);
-    lemma_pow2_mod_mod_zero (v c0) (U32.v sh) (r.len - 64);
+    lemma_pow2_mul_mod (v b0) (I64.v d) (r.len - 64);
+    lemma_pow2_mod_mod_zero (v b0) (I64.v sh) (r.len - 64 - I64.v d);
+    //! assert(v b0 * pow2 (I64.v d) % pow2 (r.len - 64) = 0);
+    lemma_pow2_mod_mod_zero (v c0) (I64.v sh) (r.len - 64);
     //! assert(v c0 % pow2 (r.len - 64) = 0);
-    lemma_mod_distr_zero (v b0 * pow2 (U32.v d)) (v c0) (pow2 (r.len - 64));
+    lemma_mod_distr_zero (v b0 * pow2 (I64.v d)) (v c0) (pow2 (r.len - 64));
     //! assert(r.limb % pow2 (r.len - 64) = 0);
     mpfr_add1sp1_gt_branch12_former_sb_lemma h a b c sh d mask;
     lemma_pow2_mod_mod r.limb (r.len - p - 1) (r.len - 64);
@@ -271,7 +271,7 @@ let mpfr_add1sp1_gt_branch1_sb_lemma h a b c sh d mask =
 
 val mpfr_add1sp1_gt_branch2_latter_sb_lemma:
     h:mem -> a:mpfr_struct -> b:mpfr_struct -> c:mpfr_struct ->
-    sh:mpfr_reg_prec_t -> d:u32 -> mask:mp_limb_t -> Lemma
+    sh:mpfr_reg_prec_t -> d:i64 -> mask:mp_limb_t -> Lemma
     (requires (mpfr_add1sp1_gt_branch2_pre_cond a b c sh d mask h))
     (ensures  (
     let r = add1sp_exact (as_reg_fp_ h b) (as_reg_fp_ h c) in
@@ -279,9 +279,9 @@ val mpfr_add1sp1_gt_branch2_latter_sb_lemma:
     let cp = c.mpfr_d in
     let b0 = Seq.index (as_seq h bp) 0 in
     let c0 = Seq.index (as_seq h cp) 0 in
-    let sb = c0 <<^ U32.(gmp_NUMB_BITS -^ d) in
-    let a0 = b0 +%^ (c0 >>^ d) in
-    (v sb <> 0) = (r.limb % pow2 (U32.v d) <> 0)))
+    let sb = c0 <<^ (int64_to_uint32 I64.(gmp_NUMB_BITS -^ d)) in
+    let a0 = b0 +%^ (c0 >>^ (int64_to_uint32 d)) in
+    (v sb <> 0) = (r.limb % pow2 (I64.v d) <> 0)))
 
 let mpfr_add1sp1_gt_branch2_latter_sb_lemma h a b c sh d mask =
     let r = add1sp_exact (as_reg_fp_ h b) (as_reg_fp_ h c) in
@@ -289,98 +289,98 @@ let mpfr_add1sp1_gt_branch2_latter_sb_lemma h a b c sh d mask =
     let cp = c.mpfr_d in
     let b0 = Seq.index (as_seq h bp) 0 in
     let c0 = Seq.index (as_seq h cp) 0 in
-    let sb = c0 <<^ U32.(gmp_NUMB_BITS -^ d) in
-    lemma_pow2_mul_mod (v c0) (64 - U32.v d) 64;
-    //! assert(v sb = (v c0 % pow2 (U32.v d)) * pow2 (64 - U32.v d));
-    let t0 = v b0 + v c0 / pow2 (U32.v d) in
-    lemma_distr_add_right (pow2 (U32.v d)) (v b0) (v c0 / pow2 (U32.v d));
-    lemma_euclidean (v c0) (pow2 (U32.v d));
-    assert(t0 * pow2 (U32.v d) + v c0 % pow2 (U32.v d) = r.limb);
-    lemma_add_mod (v c0 % pow2 (U32.v d)) t0 (pow2 (U32.v d));
-    lemma_pow2_mod_mod (v c0) (U32.v d) (U32.v d);
-    assert(v c0 % pow2 (U32.v d) = r.limb % pow2 (U32.v d));
-    lemma_mul_zero (v c0 % pow2 (U32.v d)) (pow2 (64 - U32.v d))
+    let sb = c0 <<^ (int64_to_uint32 I64.(gmp_NUMB_BITS -^ d)) in
+    lemma_pow2_mul_mod (v c0) (64 - I64.v d) 64;
+    //! assert(v sb = (v c0 % pow2 (I64.v d)) * pow2 (64 - I64.v d));
+    let t0 = v b0 + v c0 / pow2 (I64.v d) in
+    lemma_distr_add_right (pow2 (I64.v d)) (v b0) (v c0 / pow2 (I64.v d));
+    lemma_euclidean (v c0) (pow2 (I64.v d));
+    assert(t0 * pow2 (I64.v d) + v c0 % pow2 (I64.v d) = r.limb);
+    lemma_add_mod (v c0 % pow2 (I64.v d)) t0 (pow2 (I64.v d));
+    lemma_pow2_mod_mod (v c0) (I64.v d) (I64.v d);
+    assert(v c0 % pow2 (I64.v d) = r.limb % pow2 (I64.v d));
+    lemma_mul_zero (v c0 % pow2 (I64.v d)) (pow2 (64 - I64.v d))
 
 val mpfr_add1sp1_gt_branch2_sb_lemma:
     h:mem -> a:mpfr_struct -> b:mpfr_struct -> c:mpfr_struct ->
-    sh:mpfr_reg_prec_t -> d:u32 -> mask:mp_limb_t -> Lemma
+    sh:mpfr_reg_prec_t -> d:i64 -> mask:mp_limb_t -> Lemma
     (requires (mpfr_add1sp1_gt_branch2_pre_cond a b c sh d mask h))
     (ensures  (
-    let p = U32.v a.mpfr_prec in
+    let p = I64.v a.mpfr_prec in
     let r = add1sp_exact (as_reg_fp_ h b) (as_reg_fp_ h c) in
     let bp = b.mpfr_d in
     let cp = c.mpfr_d in
     let b0 = Seq.index (as_seq h bp) 0 in
     let c0 = Seq.index (as_seq h cp) 0 in
-    let sb = c0 <<^ U32.(gmp_NUMB_BITS -^ d) in
-    let a0 = b0 +%^ (c0 >>^ d) in
+    let sb = c0 <<^ (int64_to_uint32 I64.(gmp_NUMB_BITS -^ d)) in
+    let a0 = b0 +%^ (c0 >>^ (int64_to_uint32 d)) in
     let sb, a0 =
         if a0 <^ b0 then
 	    sb |^ (a0 &^ 1uL), mpfr_LIMB_HIGHBIT |^ (a0 >>^ 1ul)
 	else sb, a0 in
-    let rb = a0 &^ (mpfr_LIMB_ONE <<^ U32.(sh -^ 1ul)) in
+    let rb = a0 &^ (mpfr_LIMB_ONE <<^ (int64_to_uint32 I64.(sh -^ 1L))) in
     let sb = sb |^ ((a0 &^ mask) ^^ rb) in
     sb_def r p = (v sb <> 0)))
 
 let mpfr_add1sp1_gt_branch2_sb_lemma h a b c sh d mask = 
-    let p = U32.v a.mpfr_prec in
+    let p = I64.v a.mpfr_prec in
     let r = add1sp_exact (as_reg_fp_ h b) (as_reg_fp_ h c) in
     let bp = b.mpfr_d in
     let cp = c.mpfr_d in
     let b0 = Seq.index (as_seq h bp) 0 in
     let c0 = Seq.index (as_seq h cp) 0 in
-    let sb = c0 <<^ U32.(gmp_NUMB_BITS -^ d) in
+    let sb = c0 <<^ (int64_to_uint32 I64.(gmp_NUMB_BITS -^ d)) in
     mpfr_add1sp1_gt_branch2_latter_sb_lemma h a b c sh d mask;
-    let a0 = b0 +%^ (c0 >>^ d) in
-    lemma_add_div (v c0) (v b0) (pow2 (U32.v d));
-    lemma_pow2_mod_mod (v b0 + v c0 / pow2 (U32.v d)) 64 1;
-    //! assert((r.limb / pow2 (U32.v d)) % pow2 1 = v a0 % 2);
+    let a0 = b0 +%^ (c0 >>^ (int64_to_uint32 d)) in
+    lemma_add_div (v c0) (v b0) (pow2 (I64.v d));
+    lemma_pow2_mod_mod (v b0 + v c0 / pow2 (I64.v d)) 64 1;
+    //! assert((r.limb / pow2 (I64.v d)) % pow2 1 = v a0 % 2);
     lemma_tail_mask_value a0 1uL 1;
-    //! assert((r.limb / pow2 (U32.v d) % pow2 1 <> 0) = (v (a0 &^ 1uL) <> 0));
+    //! assert((r.limb / pow2 (I64.v d) % pow2 1 <> 0) = (v (a0 &^ 1uL) <> 0));
     mpfr_add1sp1_gt_branch12_a0_bx_lemma h a b c sh d mask;
     let sb, a0 =
         if a0 <^ b0 then begin
-	    lemma_sb_logor #r.len r.limb (r.len - 64) (U32.v d) sb (a0 &^ 1uL);
+	    lemma_sb_logor #r.len r.limb (r.len - 64) (I64.v d) sb (a0 &^ 1uL);
 	    sb |^ (a0 &^ 1uL), mpfr_LIMB_HIGHBIT |^ (a0 >>^ 1ul)
 	end else begin
 	    sb, a0
 	end in
     //! assert((r.limb % pow2 (r.len - 64) <> 0) = (v sb <> 0));
-    let rb = a0 &^ (mpfr_LIMB_ONE <<^ U32.(sh -^ 1ul)) in
+    let rb = a0 &^ (mpfr_LIMB_ONE <<^ (int64_to_uint32 I64.(sh -^ 1L))) in
     let sb' = (a0 &^ mask) ^^ rb in
     mpfr_add1sp1_gt_branch12_former_sb_lemma h a b c sh d mask;
     lemma_pow2_mod_div r.limb (r.len - p - 1) (r.len - 64);
-    //! assert((r.limb / pow2 (r.len - 64) % pow2 (U32.v sh - 1) <> 0) = (v sb' <> 0));
+    //! assert((r.limb / pow2 (r.len - 64) % pow2 (I64.v sh - 1) <> 0) = (v sb' <> 0));
     lemma_sb_logor #r.len r.limb (r.len - p - 1) (r.len - 64) sb sb'
 
 (* lemmas and implementation for mpfr_add1sp1_gt_branch1 where d >= 64 *)
 let mpfr_add1sp1_gt_branch3_pre_cond a b c sh h =
     mpfr_add1sp1_gt_pre_cond a b c sh h /\
-    I32.v b.mpfr_exp - I32.v c.mpfr_exp >= U32.v gmp_NUMB_BITS
+    I64.v b.mpfr_exp - I64.v c.mpfr_exp >= I64.v gmp_NUMB_BITS
 
 val mpfr_add1sp1_gt_branch3_value_lemma:
     h:mem -> a:mpfr_struct -> b:mpfr_struct -> c:mpfr_struct ->
     sh:mpfr_reg_prec_t -> Lemma
     (requires (mpfr_add1sp1_gt_branch3_pre_cond a b c sh h))
     (ensures  (
-    let p = U32.v a.mpfr_prec in
+    let p = I64.v a.mpfr_prec in
     let r = add1sp_exact (as_reg_fp_ h b) (as_reg_fp_ h c) in
     let r = high_mant r p in
     let bp = b.mpfr_d in
     let bx = b.mpfr_exp in
     let b0 = Seq.index (as_seq h bp) 0 in
     let a0 = b0 in
-    v a0 * pow2 (r.len - 64) = r.limb /\ I32.v bx = r.exp /\
+    v a0 * pow2 (r.len - 64) = r.limb /\ I64.v bx = r.exp /\
     v a0 >= pow2 63 /\ v a0 % pow2 (64 - p) = 0))
 
 let mpfr_add1sp1_gt_branch3_value_lemma h a b c sh =
-    let p = U32.v a.mpfr_prec in
+    let p = I64.v a.mpfr_prec in
     let r = add1sp_exact (as_reg_fp_ h b) (as_reg_fp_ h c) in
     let bp = b.mpfr_d in
     let cp = c.mpfr_d in
     let bx = b.mpfr_exp in
     let cx = c.mpfr_exp in
-    let d = I32.v bx - I32.v cx in
+    let d = I64.v bx - I64.v cx in
     let b0 = Seq.index (as_seq h bp) 0 in
     let c0 = Seq.index (as_seq h cp) 0 in
     let a0 = b0 in
@@ -404,19 +404,19 @@ val mpfr_add1sp1_gt_branch3_rb_lemma:
     sh:mpfr_reg_prec_t -> Lemma
     (requires (mpfr_add1sp1_gt_branch3_pre_cond a b c sh h))
     (ensures  (
-    let p = U32.v a.mpfr_prec in
+    let p = I64.v a.mpfr_prec in
     let r = add1sp_exact (as_reg_fp_ h b) (as_reg_fp_ h c) in
     let rb = 0uL in
     rb_def r p = (v rb <> 0)))
 
 let mpfr_add1sp1_gt_branch3_rb_lemma h a b c sh =
-    let p = U32.v a.mpfr_prec in
+    let p = I64.v a.mpfr_prec in
     let r = add1sp_exact (as_reg_fp_ h b) (as_reg_fp_ h c) in
     let bp = b.mpfr_d in
     let cp = c.mpfr_d in
     let bx = b.mpfr_exp in
     let cx = c.mpfr_exp in
-    let d = I32.v bx - I32.v cx in
+    let d = I64.v bx - I64.v cx in
     let b0 = Seq.index (as_seq h bp) 0 in
     let c0 = Seq.index (as_seq h cp) 0 in
     lemma_pow2_mul_range (v b0) d 64;
@@ -440,19 +440,19 @@ val mpfr_add1sp1_gt_branch3_sb_lemma:
     sh:mpfr_reg_prec_t -> Lemma
     (requires (mpfr_add1sp1_gt_branch3_pre_cond a b c sh h))
     (ensures  (
-    let p = U32.v a.mpfr_prec in
+    let p = I64.v a.mpfr_prec in
     let r = add1sp_exact (as_reg_fp_ h b) (as_reg_fp_ h c) in
     let sb = 1uL in
     sb_def r p = (v sb <> 0)))
 
 let mpfr_add1sp1_gt_branch3_sb_lemma h a b c sh =
-    let p = U32.v a.mpfr_prec in
+    let p = I64.v a.mpfr_prec in
     let r = add1sp_exact (as_reg_fp_ h b) (as_reg_fp_ h c) in
     let bp = b.mpfr_d in
     let cp = c.mpfr_d in
     let bx = b.mpfr_exp in
     let cx = c.mpfr_exp in
-    let d = I32.v bx - I32.v cx in
+    let d = I64.v bx - I64.v cx in
     let b0 = Seq.index (as_seq h bp) 0 in
     let c0 = Seq.index (as_seq h cp) 0 in
     lemma_pow2_mul_range (v b0) d 64;
@@ -472,16 +472,16 @@ let mpfr_add1sp1_gt_branch3_sb_lemma h a b c sh =
 
 (* pre-condition for mpfr_add1sp1_eq where b.exp = c.exp *)
 let mpfr_add1sp1_eq_pre_cond a b c sh h =
-    I32.v b.mpfr_exp = I32.v c.mpfr_exp /\
-    U32.v sh = U32.v gmp_NUMB_BITS - U32.v a.mpfr_prec /\
-    mpfr_add1sp1_any_pre_cond a b c U32.(gmp_NUMB_BITS -^ sh) h
+    I64.v b.mpfr_exp = I64.v c.mpfr_exp /\
+    I64.v sh = I64.v gmp_NUMB_BITS - I64.v a.mpfr_prec /\
+    mpfr_add1sp1_any_pre_cond a b c I64.(gmp_NUMB_BITS -^ sh) h
 
 val mpfr_add1sp1_eq_value_lemma:
     h:mem -> a:mpfr_struct -> b:mpfr_struct -> c:mpfr_struct ->
     sh:mpfr_reg_prec_t -> Lemma
     (requires (mpfr_add1sp1_eq_pre_cond a b c sh h))
     (ensures  (
-    let p = U32.v a.mpfr_prec in
+    let p = I64.v a.mpfr_prec in
     let r = add1sp_exact (as_reg_fp_ h b) (as_reg_fp_ h c) in
     let r = high_mant r p in
     let bp = b.mpfr_d in
@@ -489,39 +489,39 @@ val mpfr_add1sp1_eq_value_lemma:
     let b0 = Seq.index (as_seq h bp) 0 in
     let c0 = Seq.index (as_seq h cp) 0 in
     let a0 = (b0 >>^ 1ul) +%^ (c0 >>^ 1ul) in
-    let bx = I32.(b.mpfr_exp +^ 1l) in
-    let rb = a0 &^ (mpfr_LIMB_ONE <<^ U32.(sh -^ 1ul)) in
+    let bx = I64.(b.mpfr_exp +^ 1L) in
+    let rb = a0 &^ (mpfr_LIMB_ONE <<^ (int64_to_uint32 I64.(sh -^ 1L))) in
     let a0 = a0 ^^ rb in
-    v a0 * pow2 (r.len - 64) = r.limb /\ I32.v bx = r.exp /\
+    v a0 * pow2 (r.len - 64) = r.limb /\ I64.v bx = r.exp /\
     v a0 >= pow2 63 /\ v a0 % pow2 (64 - p) = 0))
     
 let mpfr_add1sp1_eq_value_lemma h a b c sh =
-    let p = U32.v a.mpfr_prec in
+    let p = I64.v a.mpfr_prec in
     let r = add1sp_exact (as_reg_fp_ h b) (as_reg_fp_ h c) in
     let bp = b.mpfr_d in
     let cp = c.mpfr_d in
     let b0 = Seq.index (as_seq h bp) 0 in
     let c0 = Seq.index (as_seq h cp) 0 in
     let a0 = (b0 >>^ 1ul) +%^ (c0 >>^ 1ul) in
-    lemma_pow2_mod_mod_zero (v b0) (U32.v sh) 1;
+    lemma_pow2_mod_mod_zero (v b0) (I64.v sh) 1;
     lemma_div_distr (v b0) (v c0) (pow2 1);
     //! assert(v a0 = r.limb / pow2 (r.len - 64));
     UInt.slice_left_lemma (UInt.to_vec #r.len r.limb) 64;
     //! assert(UInt.nth (v a0) p = UInt.nth #r.len r.limb p);
-    lemma_pow2_mod_div (v b0) (U32.v sh) 1;
-    lemma_pow2_mod_div (v c0) (U32.v sh) 1;
-    lemma_mod_distr_zero (v b0 / 2) (v c0 / 2) (pow2 (U32.v sh - 1));
-    //! assert(v a0 % pow2 (U32.v sh - 1) = 0);
-    lemma_mod_pow2_imp_tl_zero (v a0) (U32.v sh - 1);
+    lemma_pow2_mod_div (v b0) (I64.v sh) 1;
+    lemma_pow2_mod_div (v c0) (I64.v sh) 1;
+    lemma_mod_distr_zero (v b0 / 2) (v c0 / 2) (pow2 (I64.v sh - 1));
+    //! assert(v a0 % pow2 (I64.v sh - 1) = 0);
+    lemma_mod_pow2_imp_tl_zero (v a0) (I64.v sh - 1);
     assert(forall (i:nat{p + 1 <= i /\ i < 64}). UInt.nth (v a0) i = false);
-    let rb = a0 &^ (mpfr_LIMB_ONE <<^ U32.(sh -^ 1ul)) in
-    lemma_pow2_small_mod (U32.v sh - 1) 64;
-    //! assert(v (mpfr_LIMB_ONE <<^ U32.(sh -^ 1ul)) = pow2 (U32.v sh - 1));
-    let mask = mpfr_LIMB_ONE <<^ U32.(sh -^ 1ul) in
+    let rb = a0 &^ (mpfr_LIMB_ONE <<^ (int64_to_uint32 I64.(sh -^ 1L))) in
+    lemma_pow2_small_mod (I64.v sh - 1) 64;
+    //! assert(v (mpfr_LIMB_ONE <<^ I64.(sh -^ 1ul)) = pow2 (I64.v sh - 1));
+    let mask = mpfr_LIMB_ONE <<^ (int64_to_uint32 I64.(sh -^ 1L)) in
     lemma_bit_mask_value a0 mask p;
     lemma_bit_mask mask p;
     //! assert(forall (i:nat{p <= i /\ i < 64}). UInt.nth (v (a0 ^^ rb)) i = false);
-    lemma_tl_zero_imp_mod_pow2 (v (a0 ^^ rb)) (U32.v sh);
+    lemma_tl_zero_imp_mod_pow2 (v (a0 ^^ rb)) (I64.v sh);
     UInt.nth_lemma (UInt.shift_right (v a0) (64 - p)) (UInt.shift_right (UInt.logxor (v a0) (v rb)) (64 - p));
     //! assert(v a0 / pow2 (64 - p) = v (a0 ^^ rb) / pow2 (64 - p));
     lemma_pow2_div_div r.limb (r.len - 64) (64 - p);
@@ -541,53 +541,53 @@ val mpfr_add1sp1_eq_rb_sb_lemma:
     sh:mpfr_reg_prec_t -> Lemma
     (requires (mpfr_add1sp1_eq_pre_cond a b c sh h))
     (ensures  (
-    let p = U32.v a.mpfr_prec in
+    let p = I64.v a.mpfr_prec in
     let r = add1sp_exact (as_reg_fp_ h b) (as_reg_fp_ h c) in
     let bp = b.mpfr_d in
     let cp = c.mpfr_d in
     let b0 = Seq.index (as_seq h bp) 0 in
     let c0 = Seq.index (as_seq h cp) 0 in
     let a0 = (b0 >>^ 1ul) +%^ (c0 >>^ 1ul) in
-    let rb = a0 &^ (mpfr_LIMB_ONE <<^ U32.(sh -^ 1ul)) in
+    let rb = a0 &^ (mpfr_LIMB_ONE <<^ (int64_to_uint32 I64.(sh -^ 1L))) in
     let sb = 0uL in
     rb_def r p = (v rb <> 0) /\ sb_def r p = (v sb <> 0)))
     
 let mpfr_add1sp1_eq_rb_sb_lemma h a b c sh =
-    let p = U32.v a.mpfr_prec in
+    let p = I64.v a.mpfr_prec in
     let r = add1sp_exact (as_reg_fp_ h b) (as_reg_fp_ h c) in
     let bp = b.mpfr_d in
     let cp = c.mpfr_d in
     let b0 = Seq.index (as_seq h bp) 0 in
     let c0 = Seq.index (as_seq h cp) 0 in
     let a0 = (b0 >>^ 1ul) +%^ (c0 >>^ 1ul) in
-    lemma_pow2_mod_mod_zero (v b0) (U32.v sh) 1;
+    lemma_pow2_mod_mod_zero (v b0) (I64.v sh) 1;
     lemma_div_distr (v b0) (v c0) (pow2 1);
     //! assert(v a0 = r.limb / pow2 (r.len - 64));
     UInt.slice_left_lemma (UInt.to_vec #r.len r.limb) 64;
     //! assert(UInt.nth (v a0) p = UInt.nth #r.len r.limb p);
-    let rb = a0 &^ (mpfr_LIMB_ONE <<^ U32.(sh -^ 1ul)) in
-    lemma_pow2_small_mod (U32.v sh - 1) 64;
-    //! assert(v (mpfr_LIMB_ONE <<^ U32.(sh -^ 1ul)) = pow2 (U32.v sh - 1));
-    lemma_bit_mask_value a0 (mpfr_LIMB_ONE <<^ U32.(sh -^ 1ul)) p
+    let rb = a0 &^ (mpfr_LIMB_ONE <<^ (int64_to_uint32 I64.(sh -^ 1L))) in
+    lemma_pow2_small_mod (I64.v sh - 1) 64;
+    //! assert(v (mpfr_LIMB_ONE <<^ I64.(sh -^ 1ul)) = pow2 (I64.v sh - 1));
+    lemma_bit_mask_value a0 (mpfr_LIMB_ONE <<^ (int64_to_uint32 I64.(sh -^ 1L))) p
 
 
 (* Rounding lemmas *)
-val mpfr_add1sp1_is_even_lemma: a0:mp_limb_t -> sh:mpfr_prec_t{U32.v sh > 0 /\ U32.v sh < 64} ->
-    high:normal_fp{high.len >= 64 /\ high.prec = 64 - U32.v sh} -> Lemma
+val mpfr_add1sp1_is_even_lemma: a0:mp_limb_t -> sh:mpfr_prec_t{I64.v sh > 0 /\ I64.v sh < 64} ->
+    high:normal_fp{high.len >= 64 /\ high.prec = 64 - I64.v sh} -> Lemma
     (requires (v a0 * pow2 (high.len - 64) = high.limb))
-    (ensures  (is_even high = ((a0 &^ (mpfr_LIMB_ONE <<^ sh)) =^ 0uL)))
+    (ensures  (is_even high = ((a0 &^ (mpfr_LIMB_ONE <<^ (int64_to_uint32 sh))) =^ 0uL)))
 
 let mpfr_add1sp1_is_even_lemma a0 sh high =
-    let p = 64 - U32.v sh in
+    let p = 64 - I64.v sh in
     lemma_multiple_div (v a0) (pow2 (high.len - 64));
     assert(v a0 = high.limb / pow2 (high.len - 64));
     lemma_pow2_div_range high.limb (high.len - 64) high.len;
     slice_left_nth_lemma #high.len high.limb 64;
     assert(UInt.nth (v a0) p = UInt.nth #high.len high.limb p);
-    let gb = a0 &^ (mpfr_LIMB_ONE <<^ sh) in
-    lemma_pow2_small_mod (U32.v sh) 64;
-    //! assert(v (mpfr_LIMB_ONE <<^ sh) = pow2 (U32.v sh));
-    lemma_bit_mask_value a0 (mpfr_LIMB_ONE <<^ sh) (p - 1)
+    let gb = a0 &^ (mpfr_LIMB_ONE <<^ (int64_to_uint32 sh)) in
+    lemma_pow2_small_mod (I64.v sh) 64;
+    //! assert(v (mpfr_LIMB_ONE <<^ sh) = pow2 (I64.v sh));
+    lemma_bit_mask_value a0 (mpfr_LIMB_ONE <<^ (int64_to_uint32 sh)) (p - 1)
 
 (* perform rounding with high part of significand, rounding/sticky bit *)
 let mpfr_add1sp1_round_spec (high:normal_fp) (rb:bool) (sb:bool) (rnd_mode:mpfr_rnd_t):
