code/mpfr/MPFR.Add1sp1.fst
@@ -20,15 +20,15 @@ open MPFR.Exceptions.Lemma
 open MPFR.Add1sp1.Lemma
 
 module ST = FStar.HyperStack.ST
-module I64 = FStar.Int64
 module I32 = FStar.Int32
+module I64 = FStar.Int64
 module U32 = FStar.UInt32
 
 #set-options "--z3refresh --z3rlimit 100 --max_fuel 1 --initial_fuel 0 --max_ifuel 1 --initial_ifuel 0"
 
 (* implementations *)
 (* intermediate results *)
-private type mpfr_tmp_exp_t = x:mpfr_exp_t{I32.(x >=^ mpfr_EMIN /\ x <=^ mpfr_EMAX +^ 1l)}
+private type mpfr_tmp_exp_t = x:mpfr_exp_t{I64.(x >=^ mpfr_EMIN /\ x <=^ mpfr_EMAX +^ 1L)}
 
 private noeq type state = {
     sh:mpfr_reg_prec_t;
@@ -45,23 +45,23 @@ let mk_state sh bx rb sb = {
 }
     
 let mpfr_add1sp1_any_post_cond a b c h0 s h1 =
-    let p = U32.v a.mpfr_prec in
+    let p = I64.v a.mpfr_prec in
     live h1 a.mpfr_d /\ live h1 b.mpfr_d /\ live h1 c.mpfr_d /\
     length a.mpfr_d = 1 /\ length b.mpfr_d = 1 /\ length c.mpfr_d = 1 /\
     modifies_1 a.mpfr_d h0 h1 /\ normal_cond_ h1 a /\
-    U32.v a.mpfr_prec = U32.v b.mpfr_prec /\
-    U32.v a.mpfr_prec = U32.v c.mpfr_prec /\
+    I64.v a.mpfr_prec = I64.v b.mpfr_prec /\
+    I64.v a.mpfr_prec = I64.v c.mpfr_prec /\
     mpfr_reg_cond_ h0 b /\ mpfr_reg_cond_ h0 c /\
     (let r = add1sp_exact (as_reg_fp_ h0 b) (as_reg_fp_ h0 c) in
     as_val h1 a.mpfr_d * pow2 (r.len - 64) = (high_mant r p).limb /\
-    U32.v s.sh = U32.v gmp_NUMB_BITS - p /\
-    I32.v s.bx = (high_mant r p).exp /\
+    I64.v s.sh = I64.v gmp_NUMB_BITS - p /\
+    I64.v s.bx = (high_mant r p).exp /\
     (rb_def r p = (v s.rb <> 0)) /\
     (sb_def r p = (v s.sb <> 0)))
 
 inline_for_extraction val mpfr_add1sp1_gt_branch1:
     a:mpfr_struct -> b:mpfr_struct -> c:mpfr_struct ->
-    sh:mpfr_reg_prec_t -> d:u32 -> mask:mp_limb_t -> Stack state
+    sh:mpfr_reg_prec_t -> d:i64 -> mask:mp_limb_t -> Stack state
     (requires (fun h -> mpfr_add1sp1_gt_branch1_pre_cond a b c sh d mask h))
     (ensures  (fun h0 s h1 -> mpfr_add1sp1_any_post_cond a b c h0 s h1))
 
@@ -71,10 +71,10 @@ let mpfr_add1sp1_gt_branch1 a b c sh d mask =
     let bp = b.mpfr_d in
     let cp = c.mpfr_d in
     let bx = b.mpfr_exp in
-    let a0 = bp.(0ul) +%^ (cp.(0ul) >>^ d) in
-    let a0, bx = if a0 <^ bp.(0ul) then mpfr_LIMB_HIGHBIT |^ (a0 >>^ 1ul), I32.(bx +^ 1l)
+    let a0 = bp.(0ul) +%^ (cp.(0ul) >>^ (int64_to_uint32 d)) in
+    let a0, bx = if a0 <^ bp.(0ul) then mpfr_LIMB_HIGHBIT |^ (a0 >>^ 1ul), I64.(bx +^ 1L)
 	         else a0, bx in
-    let rb = a0 &^ (mpfr_LIMB_ONE <<^ U32.(sh -^ 1ul)) in
+    let rb = a0 &^ (mpfr_LIMB_ONE <<^ (int64_to_uint32 I64.(sh -^ 1L))) in
     let sb = (a0 &^ mask) ^^ rb in
     ap.(0ul) <- a0 &^ (lognot mask);
     mpfr_add1sp1_gt_branch12_value_lemma h a b c sh d mask;
@@ -85,7 +85,7 @@ let mpfr_add1sp1_gt_branch1 a b c sh d mask =
 
 inline_for_extraction val mpfr_add1sp1_gt_branch2:
     a:mpfr_struct -> b:mpfr_struct -> c:mpfr_struct ->
-    sh:mpfr_reg_prec_t -> d:u32 -> mask:mp_limb_t -> Stack state
+    sh:mpfr_reg_prec_t -> d:i64 -> mask:mp_limb_t -> Stack state
     (requires (fun h -> mpfr_add1sp1_gt_branch2_pre_cond a b c sh d mask h))
     (ensures  (fun h0 s h1 -> mpfr_add1sp1_any_post_cond a b c h0 s h1))
 
@@ -95,13 +95,13 @@ let mpfr_add1sp1_gt_branch2 a b c sh d mask =
     let bp = b.mpfr_d in
     let cp = c.mpfr_d in
     let bx = b.mpfr_exp in
-    let sb = cp.(0ul) <<^ U32.(gmp_NUMB_BITS -^ d) in
-    let a0 = bp.(0ul) +%^ (cp.(0ul) >>^ d) in
+    let sb = cp.(0ul) <<^ (int64_to_uint32 I64.(gmp_NUMB_BITS -^ d)) in
+    let a0 = bp.(0ul) +%^ (cp.(0ul) >>^ (int64_to_uint32 d)) in
     let sb, a0, bx =
         if a0 <^ bp.(0ul) then
-	    sb |^ (a0 &^ 1uL), mpfr_LIMB_HIGHBIT |^ (a0 >>^ 1ul), I32.(bx +^ 1l)
+	    sb |^ (a0 &^ 1uL), mpfr_LIMB_HIGHBIT |^ (a0 >>^ 1ul), I64.(bx +^ 1L)
 	else sb, a0, bx in
-    let rb = a0 &^ (mpfr_LIMB_ONE <<^ U32.(sh -^ 1ul)) in
+    let rb = a0 &^ (mpfr_LIMB_ONE <<^ (int64_to_uint32 I64.(sh -^ 1L))) in
     let sb = sb |^ ((a0 &^ mask) ^^ rb) in
     ap.(0ul) <- a0 &^ (lognot mask);
     mpfr_add1sp1_gt_branch12_value_lemma h a b c sh d mask;
@@ -139,10 +139,10 @@ inline_for_extraction val mpfr_add1sp1_gt:
 let mpfr_add1sp1_gt a b c p sh =
     let bx = b.mpfr_exp in
     let cx = c.mpfr_exp in
-    let d = int32_to_uint32 I32.(bx -^ cx) in
-    let mask = mpfr_LIMB_MASK sh in
-    if U32.(d <^ sh) then mpfr_add1sp1_gt_branch1 a b c sh d mask
-    else if U32.(d <^ gmp_NUMB_BITS) then mpfr_add1sp1_gt_branch2 a b c sh d mask
+    let d = I64.(bx -^ cx) in
+    let mask = mpfr_LIMB_MASK (int64_to_uint32 sh) in
+    if I64.(d <^ sh) then mpfr_add1sp1_gt_branch1 a b c sh d mask
+    else if I64.(d <^ gmp_NUMB_BITS) then mpfr_add1sp1_gt_branch2 a b c sh d mask
     else mpfr_add1sp1_gt_branch3 a b c sh
 
 inline_for_extraction val mpfr_add1sp1_eq:
@@ -157,8 +157,8 @@ let mpfr_add1sp1_eq a b c p sh =
     let bp = b.mpfr_d in
     let cp = c.mpfr_d in
     let a0 = (bp.(0ul) >>^ 1ul) +^ (cp.(0ul) >>^ 1ul) in
-    let bx = I32.(b.mpfr_exp +^ 1l) in
-    let rb = a0 &^ (mpfr_LIMB_ONE <<^ U32.(sh -^ 1ul)) in
+    let bx = I64.(b.mpfr_exp +^ 1L) in
+    let rb = a0 &^ (mpfr_LIMB_ONE <<^ (int64_to_uint32 I64.(sh -^ 1L))) in
     ap.(0ul) <- a0 ^^ rb;
     let sb = 0uL in
     mpfr_add1sp1_eq_value_lemma h a b c sh;
@@ -174,10 +174,10 @@ inline_for_extraction val mpfr_add1sp1_any:
 let mpfr_add1sp1_any a b c p =
     let bx = b.mpfr_exp in
     let cx = c.mpfr_exp in
-    let sh = U32.(gmp_NUMB_BITS -^ p) in
+    let sh = I64.(gmp_NUMB_BITS -^ p) in
     let h0 = ST.get() in
-    if I32.(bx =^ cx) then mpfr_add1sp1_eq a b c p sh
-    else if I32.(bx >^ cx) then mpfr_add1sp1_gt a b c p sh
+    if I64.(bx =^ cx) then mpfr_add1sp1_eq a b c p sh
+    else if I64.(bx >^ cx) then mpfr_add1sp1_gt a b c p sh
     else mpfr_add1sp1_gt a c b p sh
 
 (* rounding specifications *)
@@ -185,9 +185,9 @@ inline_for_extraction val mpfr_add_one_ulp: a:mpfr_ptr -> rnd_mode:mpfr_rnd_t ->
                              sh:mpfr_reg_prec_t -> bx:mpfr_exp_t -> Stack i32
     (requires (fun h -> 
     mpfr_live h a /\ length (as_struct h a).mpfr_d = 1 /\
-    normal_cond h a /\ mpfr_PREC_COND (U32.v (as_struct h a).mpfr_prec) /\
-    sh = U32.(gmp_NUMB_BITS -^ (as_struct h a).mpfr_prec) /\
-    bx = (as_struct h a).mpfr_exp /\ mpfr_EXP_COND (I32.v bx)))
+    normal_cond h a /\ mpfr_PREC_COND (I64.v (as_struct h a).mpfr_prec) /\
+    sh = I64.(gmp_NUMB_BITS -^ (as_struct h a).mpfr_prec) /\
+    bx = (as_struct h a).mpfr_exp /\ mpfr_EXP_COND (I64.v bx)))
     (ensures  (fun h0 t h1 -> 
     mpfr_live h1 a /\ mpfr_modifies a h0 h1 /\ mpfr_valid_cond h1 a /\
     mpfr_round2_cond (add_one_ulp (as_normal h0 a)) rnd_mode (as_fp h1 a) /\
@@ -196,23 +196,23 @@ inline_for_extraction val mpfr_add_one_ulp: a:mpfr_ptr -> rnd_mode:mpfr_rnd_t ->
 let mpfr_add_one_ulp a rnd_mode sh bx =
     let h0 = ST.get() in
     let ap = mpfr_MANT a in
-    ap.(0ul) <- ap.(0ul) +%^ (mpfr_LIMB_ONE <<^ sh);
+    ap.(0ul) <- ap.(0ul) +%^ (mpfr_LIMB_ONE <<^ (int64_to_uint32 sh));
     if ap.(0ul) =^ 0uL then begin
         ap.(0ul) <- mpfr_LIMB_HIGHBIT;
 	let h1 = ST.get() in
 	lemma_reveal_modifies_1 ap h0 h1;
 	lemma_intro_modifies_2 a ap h0 h1;
-	if I32.(bx +^ 1l <=^ mpfr_EMAX) then begin
-	    mpfr_SET_EXP a I32.(bx +^ 1l);
+	if I64.(bx +^ 1L <=^ mpfr_EMAX) then begin
+	    mpfr_SET_EXP a I64.(bx +^ 1L);
 	    let h2 = ST.get() in
-	    lemma_pow2_mod 63 (U32.v sh);
+	    lemma_pow2_mod 63 (I64.v sh);
 	    eval_abs_lt_intro_lemma (as_normal h0 a) (mpfr_max_value (as_normal h0 a).sign (as_normal h0 a).prec);
 	    eval_eq_intro_lemma (add_one_ulp (as_normal h0 a)) (as_normal h2 a);
 	    //! assert(mpfr_round2_cond (add_one_ulp (as_normal h0 a)) rnd_mode (as_fp h2 a));
 	    mpfr_modifies_trans_lemma a h0 h1 h2;
 	    mpfr_RET (mpfr_SIGN a)
 	end else begin
-	    assert(eval_abs (as_normal h0 a) == mpfr_overflow_bound (U32.v (as_struct h0 a).mpfr_prec));
+	    assert(eval_abs (as_normal h0 a) == mpfr_overflow_bound (I64.v (as_struct h0 a).mpfr_prec));
 	    let t = mpfr_overflow a rnd_mode (mpfr_SIGN a) in
 	    let h2 = ST.get() in
 	    mpfr_overflow_post_cond_lemma (add_one_ulp (as_normal h0 a)) (add_one_ulp (as_normal h0 a)).prec rnd_mode (I32.v t) (as_fp h2 a);
@@ -221,10 +221,10 @@ let mpfr_add_one_ulp a rnd_mode sh bx =
 	end
     end else begin
         let h1 = ST.get() in
-	lemma_pow2_multiple_le (v (get h0 ap 0)) 64 (U32.v sh);
-	//! assert(v (get h0 ap 0) + pow2 (U32.v sh) = v (get h1 ap 0));
-	lemma_pow2_mod (U32.v sh) (U32.v sh);
-	lemma_mod_distr_zero (v (get h0 ap 0)) (pow2 (U32.v sh)) (pow2 (U32.v sh));
+	lemma_pow2_multiple_le (v (get h0 ap 0)) 64 (I64.v sh);
+	//! assert(v (get h0 ap 0) + pow2 (I64.v sh) = v (get h1 ap 0));
+	lemma_pow2_mod (I64.v sh) (I64.v sh);
+	lemma_mod_distr_zero (v (get h0 ap 0)) (pow2 (I64.v sh)) (pow2 (I64.v sh));
         exp_impl_no_overflow_lemma (as_normal h1 a);
 	lemma_reveal_modifies_1 ap h0 h1;
 	lemma_intro_modifies_2 a ap h0 h1;
@@ -233,14 +233,14 @@ let mpfr_add_one_ulp a rnd_mode sh bx =
 
 inline_for_extraction val mpfr_add1sp1_round: a:mpfr_ptr -> rnd_mode:mpfr_rnd_t -> st:state -> Stack i32
     (requires (fun h -> mpfr_live h a /\ length (as_struct h a).mpfr_d = 1 /\ normal_cond h a /\
-    (let high = {as_normal h a with exp = I32.v st.bx} in
+    (let high = {as_normal h a with exp = I64.v st.bx} in
     let p = high.prec in
     as_val h (as_struct h a).mpfr_d * pow2 (high.len - 64) = high.limb /\
-    U32.v st.sh = U32.v gmp_NUMB_BITS - p /\
-    mpfr_EXP_COND (I32.v st.bx))))
+    I64.v st.sh = I64.v gmp_NUMB_BITS - p /\
+    mpfr_EXP_COND (I64.v st.bx))))
     (ensures  (fun h0 t h1 -> 
     mpfr_live h1 a /\ mpfr_modifies a h0 h1 /\ mpfr_valid_cond h1 a /\
-    (let high = {as_normal h0 a with exp = I32.v st.bx} in
+    (let high = {as_normal h0 a with exp = I64.v st.bx} in
     mpfr_round2_cond (mpfr_add1sp1_round_spec high (st.rb <> 0uL) (st.sb <> 0uL) rnd_mode)
                      rnd_mode (as_fp h1 a) /\
     I32.v t = mpfr_add1sp1_ternary_spec high (st.rb <> 0uL) (st.sb <> 0uL) rnd_mode)))
@@ -255,7 +255,8 @@ let mpfr_add1sp1_round a rnd_mode st =
     mpfr_round2_cond_refl_lemma (as_normal h1 a) rnd_mode;
     if (st.rb =^ 0uL && st.sb =^ 0uL) then mpfr_RET 0l
     else if (MPFR_RNDN? rnd_mode) then
-        if (st.rb =^ 0uL || (st.sb =^ 0uL && ((a0 &^ (mpfr_LIMB_ONE <<^ st.sh)) =^ 0uL))) then
+        if (st.rb =^ 0uL || (st.sb =^ 0uL && 
+	                   ((a0 &^ (mpfr_LIMB_ONE <<^ (int64_to_uint32 st.sh))) =^ 0uL))) then
 	    mpfr_RET (mpfr_NEG_SIGN (mpfr_SIGN a))
 	else mpfr_add_one_ulp a rnd_mode st.sh st.bx
     else if mpfr_IS_LIKE_RNDZ rnd_mode (mpfr_IS_NEG a) then
@@ -273,7 +274,7 @@ val mpfr_add1sp1: a:mpfr_ptr -> b:mpfr_ptr -> c:mpfr_ptr ->
         length (as_struct h a).mpfr_d = 1 /\
         length (as_struct h b).mpfr_d = 1 /\ length (as_struct h c).mpfr_d = 1 /\
         (* Functional correctness *)
-        U32.v p > 0 /\ U32.v p < 64 /\ p = (as_struct h a).mpfr_prec /\
+        I64.v p > 0 /\ I64.v p < 64 /\ p = (as_struct h a).mpfr_prec /\
         p = (as_struct h b).mpfr_prec /\ p = (as_struct h c).mpfr_prec /\
         (as_struct h a).mpfr_sign = (as_struct h b).mpfr_sign /\
         mpfr_valid_cond h a /\ mpfr_reg_cond h b /\ mpfr_reg_cond h c))
@@ -285,7 +286,7 @@ val mpfr_add1sp1: a:mpfr_ptr -> b:mpfr_ptr -> c:mpfr_ptr ->
         mpfr_disjoint_or_equal h1 b c /\ mpfr_modifies a h0 h1 /\
         (* Functional correctness *)
         mpfr_valid_cond h1 a /\ 
-        mpfr_round_cond exact (U32.v p) rnd_mode (as_fp h1 a) /\
+        mpfr_round_cond exact (I64.v p) rnd_mode (as_fp h1 a) /\
         mpfr_ternary_cond (I32.v t) exact (as_fp h1 a)))
 
 let mpfr_add1sp1 a b c rnd_mode p =
@@ -297,17 +298,17 @@ let mpfr_add1sp1 a b c rnd_mode p =
     let h1 = ST.get() in
     lemma_reveal_modifies_1 (mpfr_MANT a) h0 h1;
     lemma_intro_modifies_2 a (mpfr_MANT a) h0 h1;
-    if I32.(st.bx >^ mpfr_EMAX) then begin
+    if I64.(st.bx >^ mpfr_EMAX) then begin
         let s = mpfr_SIGN a in
         let t = mpfr_overflow a rnd_mode (mpfr_SIGN a) in
 	let h2 = ST.get() in
-	mpfr_overflow_post_cond_lemma (add1sp_exact (as_reg_fp h0 b) (as_reg_fp h0 c)) (U32.v (as_struct h0 a).mpfr_prec) rnd_mode (I32.v t) (as_fp h2 a);
+	mpfr_overflow_post_cond_lemma (add1sp_exact (as_reg_fp h0 b) (as_reg_fp h0 c)) (I64.v (as_struct h0 a).mpfr_prec) rnd_mode (I32.v t) (as_fp h2 a);
 	mpfr_modifies_trans_lemma a h0 h1 h2;
 	t
     end else begin
         let t = mpfr_add1sp1_round a rnd_mode st in
 	let h2 = ST.get() in
-	mpfr_add1sp1_round_post_cond_lemma (add1sp_exact (as_reg_fp h0 b) (as_reg_fp h0 c)) (U32.v (as_struct h0 a).mpfr_prec) (as_normal_ h1 ({as_struct h1 a with mpfr_exp = st.bx})) (st.rb <> 0uL) (st.sb <> 0uL) rnd_mode (I32.v t) (as_fp h2 a);
+	mpfr_add1sp1_round_post_cond_lemma (add1sp_exact (as_reg_fp h0 b) (as_reg_fp h0 c)) (I64.v (as_struct h0 a).mpfr_prec) (as_normal_ h1 ({as_struct h1 a with mpfr_exp = st.bx})) (st.rb <> 0uL) (st.sb <> 0uL) rnd_mode (I32.v t) (as_fp h2 a);
 	mpfr_modifies_trans_lemma a h0 h1 h2;
 	t
     end
