code/mpfr/MPFR.Lib.fst
@@ -6,9 +6,11 @@ open FStar.HyperStack
 open FStar.HyperStack.ST
 open FStar.Buffer
 open FStar.UInt64
+open FStar.Int.Cast
 
 module ST = FStar.HyperStack.ST
 module I32 = FStar.Int32
+module I64 = FStar.Int64
 module U32 = FStar.UInt32
 
 open MPFR.Maths
@@ -22,6 +24,7 @@ include MPFR.RoundingMode
 
 // GENERIC LIBRARY DEFINITIONS
 type i32 = FStar.Int32.t
+type i64 = FStar.Int64.t
 type u32 = FStar.UInt32.t
 type u64 = FStar.UInt64.t
 
@@ -29,8 +32,8 @@ inline_for_extraction let mpfr_SIGN_POS = 1l
 inline_for_extraction let mpfr_SIGN_NEG = -1l
 
 type mpfr_sign_t = s:i32{s = mpfr_SIGN_NEG \/ s = mpfr_SIGN_POS}
-type mpfr_prec_t = p:u32{U32.v p > 0}
-type mpfr_exp_t  = i32
+type mpfr_prec_t = p:i64{I64.v p > 0}
+type mpfr_exp_t  = i64
 type mp_limb_t = u64
 
 noeq type mpfr_struct = {
@@ -54,42 +57,63 @@ let as_struct h (a:mpfr_ptr) = Seq.index (as_seq h a) 0
 
 (* range settings *)
 (* precision *)
-let gmp_NUMB_BITS = 64ul
-val mpfr_PREC_MIN: p:u32{U32.v p = mpfr_PREC_MIN_spec}
-let mpfr_PREC_MIN = 1ul
-val mpfr_PREC_MAX: p:u32{U32.v p = mpfr_PREC_MAX_spec}
-let mpfr_PREC_MAX = 0x7ffffffful // Note: 0x7ffffefful in original code
+val gmp_NUMB_BITS: x:i64{I64.v x = gnb}
+let gmp_NUMB_BITS = 64L
+val mpfr_PREC_MIN: p:i64{I64.v p = mpfr_PREC_MIN_spec}
+let mpfr_PREC_MIN = 1L
+val mpfr_PREC_MAX: p:i64{I64.v p = mpfr_PREC_MAX_spec}
+let mpfr_PREC_MAX = 0x7ffffffffffffeffL
 
 (* exponent *)
-inline_for_extraction val mpfr_EXP_MIN: x:i32{I32.v x = -pow2 31}
-inline_for_extraction let mpfr_EXP_MIN = assert_norm(-0x80000000 = -pow2 31); -0x80000000l
-inline_for_extraction val mpfr_EXP_MAX: x:i32{I32.v x = pow2 31 - 1}
-inline_for_extraction let mpfr_EXP_MAX = assert_norm(0x7fffffff = pow2 31 - 1); 0x7fffffffl
-inline_for_extraction let mpfr_EXP_ZERO = I32.(mpfr_EXP_MIN +^ 1l)
-inline_for_extraction let mpfr_EXP_NAN  = I32.(mpfr_EXP_MIN +^ 2l)
-inline_for_extraction let mpfr_EXP_INF  = I32.(mpfr_EXP_MIN +^ 3l)
+val mpfr_EXP_MAX:  x:i64{I64.v x = pow2 63 - 1}
+let mpfr_EXP_MAX =
+    assert_norm(0x7fffffffffffffff = pow2 63 - 1);
+    0x7fffffffffffffffL
 
-inline_for_extraction val mpfr_EXP_INVALID: x:i32{I32.v x = pow2 30}
-inline_for_extraction let mpfr_EXP_INVALID = assert_norm(0x40000000 = pow2 30); 0x40000000l
-val mpfr_EMIN: x:i32{I32.v x = mpfr_EMIN_spec}
-let mpfr_EMIN = I32.(1l -^ mpfr_EXP_INVALID)
-val mpfr_EMAX: x:i32{I32.v x = mpfr_EMAX_spec}
-let mpfr_EMAX = I32.(mpfr_EXP_INVALID -^ 1l)
+val mpfr_EXP_ZERO: x:i64{I64.v x = 0 - I64.v mpfr_EXP_MAX}
+let mpfr_EXP_ZERO = 
+    assert_norm(-0x7fffffffffffffff = 1 - pow2 63);
+    -0x7fffffffffffffffL
+
+val mpfr_EXP_NAN:  x:i64{I64.v x = 1 - I64.v mpfr_EXP_MAX}
+let mpfr_EXP_NAN  = 
+    assert_norm(-0x7ffffffffffffffe = 2 - pow2 63);
+    -0x7ffffffffffffffeL
+
+val mpfr_EXP_INF:  x:i64{I64.v x = 2 - I64.v mpfr_EXP_MAX}
+let mpfr_EXP_INF  =
+    assert_norm(-0x7ffffffffffffffd = 3 - pow2 63);
+    -0x7ffffffffffffffdL
+
+val mpfr_EXP_INVALID: x:i64{I64.v x = pow2 62}
+let mpfr_EXP_INVALID =
+    assert_norm(0x4000000000000000 = pow2 62);
+    0x4000000000000000L
+
+val mpfr_EMIN: x:i64{I64.v x = mpfr_EMIN_spec}
+let mpfr_EMIN = 
+    assert_norm(-0x3fffffffffffffff = 1 - pow2 62);
+    -0x3fffffffffffffffL
+
+val mpfr_EMAX: x:i64{I64.v x = mpfr_EMAX_spec}
+let mpfr_EMAX = 
+    assert_norm(0x3fffffffffffffff = pow2 62 - 1);
+    0x3fffffffffffffffL
 
 (* validity and regularity *)
-type mpfr_reg_prec_t = p:u32{mpfr_PREC_COND (U32.v p)}
-type mpfr_reg_exp_t  = x:i32{mpfr_EXP_COND (I32.v x)}
+type mpfr_reg_prec_t = p:i64{mpfr_PREC_COND (I64.v p)}
+type mpfr_reg_exp_t  = x:i64{mpfr_EXP_COND (I64.v x)}
 
 (* First bit is 1 *)
 let mpfr_d_valn_cond (m:mp_limb_t): GTot Type0 =
     v m >= pow2 63
 
 (* Ending bits are 0 *)
-let mpfr_d_val0_cond (m:mp_limb_t) (p:mpfr_prec_t{U32.v p > 0}): GTot Type0 =
-    v m % pow2 (prec_to_len (U32.v p) - U32.v p) = 0
+let mpfr_d_val0_cond (m:mp_limb_t) (p:mpfr_prec_t{I64.v p > 0}): GTot Type0 =
+    v m % pow2 (prec_to_len (I64.v p) - I64.v p) = 0
 
 let prec_len_cond_ h (s:mpfr_struct): GTot Type0 =
-    prec_to_len (U32.v s.mpfr_prec) = length s.mpfr_d * 64
+    prec_to_len (I64.v s.mpfr_prec) = length s.mpfr_d * gnb
 
 let prec_len_cond h (a:mpfr_ptr): GTot Type0 = prec_len_cond_ h (as_struct h a)
 
@@ -108,12 +132,12 @@ let singular_cond h (a:mpfr_ptr): GTot Type0 = singular_cond_ h (as_struct h a)
 
 let mpfr_reg_cond_ h (s:mpfr_struct): GTot Type0 =
     normal_cond_ h s /\
-    mpfr_PREC_COND (U32.v s.mpfr_prec) /\ mpfr_EXP_COND (I32.v s.mpfr_exp)
+    mpfr_PREC_COND (I64.v s.mpfr_prec) /\ mpfr_EXP_COND (I64.v s.mpfr_exp)
 
 let mpfr_reg_cond h (a:mpfr_ptr): GTot Type0 = mpfr_reg_cond_ h (as_struct h a)
 
 let mpfr_valid_cond_ h (s:mpfr_struct): GTot Type0 =
-    mpfr_PREC_COND (U32.v s.mpfr_prec) /\ 
+    mpfr_PREC_COND (I64.v s.mpfr_prec) /\ 
     (singular_cond_ h s \/ mpfr_reg_cond_ h s)
 
 let mpfr_valid_cond h (a:mpfr_ptr): GTot Type0 = mpfr_valid_cond_ h (as_struct h a)
@@ -164,16 +188,16 @@ let rec valn_cond_lemma s =
         lemma_pow2_mul (Seq.length s * 64 - 65) 64
     end
 
-val val0_cond_lemma: s:Seq.seq u64 -> p:mpfr_prec_t{U32.v p > 0} -> Lemma
-    (requires  (prec_to_len (U32.v p) = Seq.length s * 64 /\
+val val0_cond_lemma: s:Seq.seq u64 -> p:mpfr_prec_t{I64.v p > 0} -> Lemma
+    (requires  (prec_to_len (I64.v p) = Seq.length s * 64 /\
                 mpfr_d_val0_cond (Seq.index s 0) p))
-    (ensures   (to_val s % pow2 (Seq.length s * 64 - U32.v p) = 0))
-    (decreases (U32.v p))
+    (ensures   (to_val s % pow2 (Seq.length s * 64 - I64.v p) = 0))
+    (decreases (I64.v p))
     
 let val0_cond_lemma s p =
-    lemma_pow2_mod 64 (Seq.length s * 64 - U32.v p);
-    lemma_mul_mod_zero (to_val (Seq.slice s 1 (Seq.length s))) (pow2 64) (pow2 (Seq.length s * 64 - U32.v p));
-    lemma_mod_distr_zero (v (Seq.index s 0)) (to_val (Seq.slice s 1 (Seq.length s)) * pow2 64) (pow2 (Seq.length s * 64 - U32.v p))
+    lemma_pow2_mod 64 (Seq.length s * 64 - I64.v p);
+    lemma_mul_mod_zero (to_val (Seq.slice s 1 (Seq.length s))) (pow2 64) (pow2 (Seq.length s * 64 - I64.v p));
+    lemma_mod_distr_zero (v (Seq.index s 0)) (to_val (Seq.slice s 1 (Seq.length s)) * pow2 64) (pow2 (Seq.length s * 64 - I64.v p))
 
 let as_val h (b:buffer mp_limb_t) = to_val (as_seq h b)
 
@@ -182,8 +206,8 @@ val as_normal_: h:mem -> s:mpfr_struct{normal_cond_ h s} -> GTot normal_fp
 
 let as_normal_ h s =
     let sign = I32.v s.mpfr_sign in
-    let prec = U32.v s.mpfr_prec in
-    let exp  = I32.v s.mpfr_exp  in
+    let prec = I64.v s.mpfr_prec in
+    let exp  = I64.v s.mpfr_exp  in
     let limb = as_val h s.mpfr_d in
     let l    = length s.mpfr_d in
     assert(prec_to_len prec = l * 64);
@@ -198,7 +222,7 @@ let as_reg_fp_ h (s:mpfr_struct{mpfr_reg_cond_ h s}): GTot mpfr_reg_fp = as_norm
 let as_reg_fp h (a:mpfr_ptr{mpfr_reg_cond h a}) = as_reg_fp_ h (as_struct h a)
 
 let as_fp_ h (s:mpfr_struct{mpfr_valid_cond_ h s}): GTot mpfr_fp =
-    let init = mk_fp_struct (I32.v s.mpfr_sign) (U32.v s.mpfr_prec) 0 0 (length s.mpfr_d * 64) MPFR_NAN in
+    let init = mk_fp_struct (I32.v s.mpfr_sign) (I64.v s.mpfr_prec) 0 0 (length s.mpfr_d * 64) MPFR_NAN in
     if s.mpfr_exp = mpfr_EXP_NAN then init
     else if s.mpfr_exp = mpfr_EXP_INF then {init with flag = MPFR_INF}
     else if s.mpfr_exp = mpfr_EXP_ZERO then {init with flag = MPFR_ZERO}
@@ -239,7 +263,7 @@ let mpfr_PREC x =
     f.mpfr_prec
 
 inline_for_extraction val mpfr_GET_PREC: x:mpfr_ptr -> Stack mpfr_reg_prec_t 
-    (requires (fun h -> mpfr_live h x /\ mpfr_PREC_COND (U32.v (as_struct h x).mpfr_prec)))
+    (requires (fun h -> mpfr_live h x /\ mpfr_PREC_COND (I64.v (as_struct h x).mpfr_prec)))
     (ensures  (fun h0 r h1 -> mpfr_live h1 x /\ h0 == h1 /\
                           r = (as_struct h1 x).mpfr_prec))
 let mpfr_GET_PREC x =
@@ -338,20 +362,20 @@ inline_for_extraction val mpfr_MANT: x:mpfr_ptr -> Stack (buffer mp_limb_t)
 let mpfr_MANT x = 
     (x.(0ul)).mpfr_d
 
-inline_for_extraction val mpn_ZERO: b:buffer mp_limb_t -> l:u32 -> Stack unit
-    (requires (fun h -> live h b /\ length b >= U32.v l))
+inline_for_extraction val mpn_ZERO: b:buffer mp_limb_t -> l:i64 -> Stack unit
+    (requires (fun h -> live h b /\ I64.v l >= 0 /\ length b >= I64.v l))
     (ensures  (fun h0 _ h1 ->
         live h1 b /\ modifies_1 b h0 h1 /\
-        (forall (i:nat{i < U32.v l}). Seq.index (as_seq h1 b) i = 0uL) /\
-        (forall (i:nat{i >= U32.v l /\ i < length b}). Seq.index (as_seq h1 b) i = Seq.index (as_seq h0 b) i) /\
-        to_val (Seq.slice (as_seq h1 b) 0 (U32.v l)) = 0))
+        (forall (i:nat{i < I64.v l}). Seq.index (as_seq h1 b) i = 0uL) /\
+        (forall (i:nat{i >= I64.v l /\ i < length b}). Seq.index (as_seq h1 b) i = Seq.index (as_seq h0 b) i) /\
+        to_val (Seq.slice (as_seq h1 b) 0 (I64.v l)) = 0))
 
 let rec mpn_ZERO b l =
-    if U32.(l =^ 0ul) then () else begin
-        b.(U32.(l -^ 1ul)) <- 0uL;
-        mpn_ZERO b U32.(l -^ 1ul);
+    if I64.(l =^ 0L) then () else begin
+        b.(int64_to_uint32 (I64.(l -^ 1L))) <- 0uL;
+        mpn_ZERO b I64.(l -^ 1L);
 	let h = ST.get() in
-	to_val_left_slice_lemma (Seq.slice (as_seq h b) 0 (U32.v l))
+	to_val_left_slice_lemma (Seq.slice (as_seq h b) 0 (I64.v l))
     end
 
 (* useful functions *)
@@ -360,20 +384,20 @@ val mpfr_RET: t:i32 -> Stack i32
     (ensures  (fun h0 r h1 -> h0 == h1 /\ r = t))
 let mpfr_RET t = t
 
-inline_for_extraction val mpfr_LAST_LIMB: x:mpfr_ptr -> Stack u32
-    (requires (fun h -> mpfr_live h x /\ mpfr_PREC_COND (U32.v (as_struct h x).mpfr_prec)))
+inline_for_extraction val mpfr_LAST_LIMB: x:mpfr_ptr -> Stack i64
+    (requires (fun h -> mpfr_live h x /\ mpfr_PREC_COND (I64.v (as_struct h x).mpfr_prec)))
     (ensures  (fun h0 r h1 -> mpfr_live h1 x /\ h0 == h1 /\
-                           (U32.v r + 1) * 64 = prec_to_len (U32.v (as_struct h1 x).mpfr_prec)))
+                           (I64.v r + 1) * 64 = prec_to_len (I64.v (as_struct h1 x).mpfr_prec)))
 
 let mpfr_LAST_LIMB x =
-    U32.((mpfr_GET_PREC x -^ 1ul) /^ gmp_NUMB_BITS)
+    I64.((mpfr_GET_PREC x -^ 1L) /^ gmp_NUMB_BITS)
 
-inline_for_extraction val mpfr_LIMB_SIZE: x:mpfr_ptr -> Stack u32
-    (requires (fun h -> mpfr_live h x /\ mpfr_PREC_COND (U32.v (as_struct h x).mpfr_prec)))
+inline_for_extraction val mpfr_LIMB_SIZE: x:mpfr_ptr -> Stack i64
+    (requires (fun h -> mpfr_live h x /\ mpfr_PREC_COND (I64.v (as_struct h x).mpfr_prec)))
     (ensures  (fun h0 r h1 -> mpfr_live h1 x /\ h0 == h1 /\
-                           U32.v r * 64 = prec_to_len (U32.v (as_struct h1 x).mpfr_prec)))
+                           I64.v r * 64 = prec_to_len (I64.v (as_struct h1 x).mpfr_prec)))
 
-let mpfr_LIMB_SIZE x = U32.(mpfr_LAST_LIMB x +^ 1ul)
+let mpfr_LIMB_SIZE x = I64.(mpfr_LAST_LIMB x +^ 1L)
 
 (* special value *)
 inline_for_extraction let mpfr_LIMB_ONE = 1uL
@@ -395,39 +419,40 @@ let mpfr_LIMB_MAX =
     0xffffffffffffffffuL
 
 (* set special value *)
-inline_for_extraction val mpfr_setmax_rec: x:mpfr_ptr -> i:u32 -> Stack unit
+inline_for_extraction val mpfr_setmax_rec: x:mpfr_ptr -> i:i64 -> Stack unit
     (requires (fun h -> 
         let p = (as_struct h x).mpfr_prec in
-        mpfr_live h x /\ U32.v i < length (as_struct h x).mpfr_d /\ mpfr_PREC_COND (U32.v p)))
+        mpfr_live h x /\ I64.v i >= 0 /\
+	I64.v i < length (as_struct h x).mpfr_d /\ mpfr_PREC_COND (I64.v p)))
     (ensures  (fun h0 _ h1 -> 
         let p = (as_struct h0 x).mpfr_prec in
         mpfr_live h1 x /\ mpfr_modifies x h0 h1 /\
         (as_struct h1 x).mpfr_sign = (as_struct h0 x).mpfr_sign /\
         (as_struct h1 x).mpfr_exp = (as_struct h0 x).mpfr_exp /\
         (let xm = as_seq h1 (as_struct h1 x).mpfr_d in
-        v (Seq.index xm 0) = pow2 64 - pow2 (prec_to_len (U32.v p) - U32.v p) /\
-        (forall (j:nat{j > 0 /\ j <= U32.v i}). v (Seq.index xm j) = pow2 64 - 1))))
+        v (Seq.index xm 0) = pow2 64 - pow2 (prec_to_len (I64.v p) - I64.v p) /\
+        (forall (j:nat{j > 0 /\ j <= I64.v i}). v (Seq.index xm j) = pow2 64 - 1))))
 
 let rec mpfr_setmax_rec x i =
     let mant = mpfr_MANT x in
-    if i = 0ul then begin
+    if i = 0L then begin
         let p = mpfr_GET_PREC x in
 	let l = mpfr_LIMB_SIZE x in
 	let h0 = ST.get() in
-	mant.(i) <- mpfr_LIMB_MAX <<^ U32.(l *^ gmp_NUMB_BITS -^ p);
-	lemma_distr_sub_left (pow2 (prec_to_len (U32.v p) - U32.v p)) (pow2 64) 1;
-	lemma_pow2_mul 64 (prec_to_len (U32.v p) - U32.v p);
-	lemma_mod_distr_sub (pow2 (64 + prec_to_len (U32.v p) - U32.v p)) (pow2 (prec_to_len (U32.v p) - U32.v p)) (pow2 64);
-	lemma_pow2_mod (64 + prec_to_len (U32.v p) - U32.v p) 64;
-	lemma_pow2_lt (prec_to_len (U32.v p) - U32.v p) 64;
-	lemma_small_mod (pow2 (prec_to_len (U32.v p) - U32.v p)) (pow2 64);
-	//! assert(v mant.(i) = pow2 64 - pow2 (prec_to_len (U32.v p) - U32.v p));
+	mant.(int64_to_uint32 i) <- mpfr_LIMB_MAX <<^ (int64_to_uint32 I64.(l *^ gmp_NUMB_BITS -^ p));
+	lemma_distr_sub_left (pow2 (prec_to_len (I64.v p) - I64.v p)) (pow2 64) 1;
+	lemma_pow2_mul 64 (prec_to_len (I64.v p) - I64.v p);
+	lemma_mod_distr_sub (pow2 (64 + prec_to_len (I64.v p) - I64.v p)) (pow2 (prec_to_len (I64.v p) - I64.v p)) (pow2 64);
+	lemma_pow2_mod (64 + prec_to_len (I64.v p) - I64.v p) 64;
+	lemma_pow2_lt (prec_to_len (I64.v p) - I64.v p) 64;
+	lemma_small_mod (pow2 (prec_to_len (I64.v p) - I64.v p)) (pow2 64);
+	//! assert(v mant.(i) = pow2 64 - pow2 (prec_to_len (I64.v p) - I64.v p));
 	let h1 = ST.get() in
 	lemma_reveal_modifies_1 (mpfr_MANT x) h0 h1;
 	lemma_intro_modifies_2 x (mpfr_MANT x) h0 h1
     end else begin
-	mpfr_setmax_rec x U32.(i -^ 1ul);
-        mant.(i) <- mpfr_LIMB_MAX
+	mpfr_setmax_rec x I64.(i -^ 1L);
+        mant.(int64_to_uint32 i) <- mpfr_LIMB_MAX
     end
 
 val to_val_setmax_lemma: s:Seq.seq u64{Seq.length s > 0} -> sh:nat{sh < 64} -> Lemma
@@ -447,8 +472,8 @@ let rec to_val_setmax_lemma s sh =
 val mpfr_setmax: x:mpfr_ptr -> Stack unit
     (requires (fun h -> 
         let p = (as_struct h x).mpfr_prec in
-        let l = U32.((p -^ 1ul) /^ 64ul +^ 1ul) in
-        mpfr_live h x /\ mpfr_PREC_COND (U32.v p) /\ length (as_struct h x).mpfr_d = U32.v l))
+        let l = I64.((p -^ 1L) /^ 64L +^ 1L) in
+        mpfr_live h x /\ mpfr_PREC_COND (I64.v p) /\ length (as_struct h x).mpfr_d = I64.v l))
     (ensures  (fun h0 _ h1 -> 
         mpfr_live h1 x /\ mpfr_modifies x h0 h1 /\
         (as_struct h1 x).mpfr_sign = (as_struct h0 x).mpfr_sign /\
@@ -462,7 +487,7 @@ let mpfr_setmax x =
     let h = ST.get() in
     let p = mpfr_GET_PREC x in
     let l = mpfr_LIMB_SIZE x in
-    let sh = prec_to_len (U32.v p) - U32.v p in
+    let sh = prec_to_len (I64.v p) - I64.v p in
     lemma_pow2_double 63;
     lemma_pow2_le sh 63;
     //! assert(pow2 64 - pow2 sh >= pow2 63);
@@ -489,8 +514,8 @@ let rec to_val_setmin_lemma s =
 val mpfr_setmin: x:mpfr_ptr -> Stack unit
     (requires (fun h -> 
         let p = (as_struct h x).mpfr_prec in
-        let l = U32.((p -^ 1ul) /^ 64ul +^ 1ul) in
-        mpfr_live h x /\ mpfr_PREC_COND (U32.v p) /\ length (as_struct h x).mpfr_d = U32.v l))
+        let l = I64.((p -^ 1L) /^ 64L +^ 1L) in
+        mpfr_live h x /\ mpfr_PREC_COND (I64.v p) /\ length (as_struct h x).mpfr_d = I64.v l))
     (ensures  (fun h0 _ h1 -> 
         mpfr_live h1 x /\ mpfr_modifies x h0 h1 /\
         (as_struct h1 x).mpfr_sign = (as_struct h0 x).mpfr_sign /\
@@ -502,10 +527,10 @@ let mpfr_setmin x =
     mpfr_SET_EXP x mpfr_EMIN;
     let xn = mpfr_LAST_LIMB x in
     let xp = mpfr_MANT x in
-    xp.(xn) <- mpfr_LIMB_HIGHBIT;
+    xp.(int64_to_uint32 xn) <- mpfr_LIMB_HIGHBIT;
     mpn_ZERO xp xn;
     let h = ST.get() in
-    lemma_pow2_mod 63 (prec_to_len (U32.v ((as_struct h x).mpfr_prec)) - U32.v ((as_struct h x).mpfr_prec));
+    lemma_pow2_mod 63 (prec_to_len (I64.v ((as_struct h x).mpfr_prec)) - I64.v ((as_struct h x).mpfr_prec));
     //! assert((pow2 63) % (pow2 sh) = 0);
     valn_cond_lemma (as_seq h (as_struct h x).mpfr_d);
     val0_cond_lemma (as_seq h (as_struct h x).mpfr_d) (as_struct h x).mpfr_prec;
