code/mpfr/MPFR.Mul_1.fst
@@ -28,13 +28,13 @@ module U32 = FStar.UInt32
 
 open FStar.Mul
 
-private type mpfr_tmp_exp_t = x:mpfr_exp_t{I32.(x >=^ mpfr_EMIN -^ 1l /\ x <=^ mpfr_EMAX)}
+private type mpfr_tmp_exp_t = x:mpfr_exp_t{I64.(x >=^ mpfr_EMIN -^ 1L /\ x <=^ mpfr_EMAX)}
 
 inline_for_extraction val mpfr_add_one_ulp: a:mpfr_ptr -> rnd_mode:mpfr_rnd_t -> sh:mpfr_prec_t -> ax:mpfr_tmp_exp_t ->
     Stack i32
     (requires (fun h ->
         mpfr_live h a /\ length (as_struct h a).mpfr_d = 1 /\
-	U32.v sh + U32.v (as_struct h a).mpfr_prec = 64 /\
+	I64.v sh + I64.v (as_struct h a).mpfr_prec = 64 /\
 	normal_cond h a))
     (ensures  (fun h0 t h1 ->
         mpfr_live h1 a /\ mpfr_modifies a h0 h1))
@@ -42,21 +42,21 @@ inline_for_extraction val mpfr_add_one_ulp: a:mpfr_ptr -> rnd_mode:mpfr_rnd_t ->
 let mpfr_add_one_ulp a rnd_mode sh ax =
     let h0 = ST.get() in
     let ap = mpfr_MANT a in
-    ap.(0ul) <- ap.(0ul) +%^ (mpfr_LIMB_ONE <<^ sh);
+    ap.(0ul) <- ap.(0ul) +%^ (mpfr_LIMB_ONE <<^ (int64_to_uint32 sh));
     let h1 = ST.get() in
     lemma_reveal_modifies_1 ap h0 h1;
     lemma_intro_modifies_2 a ap h0 h1;
     if ap.(0ul) =^ 0uL then begin
         ap.(0ul) <- mpfr_LIMB_HIGHBIT;
-	if I32.(ax +^ 1l >^ mpfr_EMAX) then mpfr_overflow a rnd_mode (mpfr_SIGN a)
-	else (mpfr_SET_EXP a I32.(ax +^ 1l); mpfr_RET (mpfr_SIGN a))
+	if I64.(ax +^ 1L >^ mpfr_EMAX) then mpfr_overflow a rnd_mode (mpfr_SIGN a)
+	else (mpfr_SET_EXP a I64.(ax +^ 1L); mpfr_RET (mpfr_SIGN a))
     end else mpfr_RET (mpfr_SIGN a)
 
 inline_for_extraction val mpfr_mul_1_rounding: a:mpfr_ptr -> sh:mpfr_prec_t -> ax:mpfr_tmp_exp_t -> 
     rb:mp_limb_t -> sb:mp_limb_t -> rnd_mode:mpfr_rnd_t -> Stack i32
     (requires (fun h ->
         mpfr_live h a /\ length (as_struct h a).mpfr_d = 1 /\
-	U32.v sh + U32.v (as_struct h a).mpfr_prec = 64 /\
+	I64.v sh + I64.v (as_struct h a).mpfr_prec = 64 /\
 	normal_cond_ h ({as_struct h a with mpfr_exp = ax})))
     (ensures  (fun h0 t h1 ->
         mpfr_live h1 a /\ mpfr_modifies a h0 h1))
@@ -69,7 +69,7 @@ let mpfr_mul_1_rounding a sh ax rb sb rnd_mode =
     let h1 = ST.get() in
     if rb =^ 0uL && sb =^ 0uL then mpfr_RET 0l
     else if MPFR_RNDN? rnd_mode then
-        if (rb =^ 0uL || (sb =^ 0uL && ((a0 &^ (mpfr_LIMB_ONE <<^ sh)) =^ 0uL))) then
+        if (rb =^ 0uL || (sb =^ 0uL && ((a0 &^ (mpfr_LIMB_ONE <<^ (int64_to_uint32 sh))) =^ 0uL))) then
 	    mpfr_RET (mpfr_NEG_SIGN (mpfr_SIGN a))
 	else mpfr_add_one_ulp a rnd_mode sh ax
     else if mpfr_IS_LIKE_RNDZ rnd_mode (mpfr_IS_NEG a) then 
@@ -80,7 +80,7 @@ inline_for_extraction val mpfr_mul_1_round: a:mpfr_ptr -> sh:mpfr_prec_t -> ax:m
     rb:mp_limb_t -> sb:mp_limb_t -> mask:mp_limb_t -> rnd_mode:mpfr_rnd_t -> Stack i32
     (requires (fun h ->
         mpfr_live h a /\ length (as_struct h a).mpfr_d = 1 /\
-	U32.v sh + U32.v (as_struct h a).mpfr_prec = 64 /\
+	I64.v sh + I64.v (as_struct h a).mpfr_prec = 64 /\
 	normal_cond_ h ({as_struct h a with mpfr_exp = ax})))
     (ensures  (fun h0 t h1 ->
         mpfr_live h1 a /\ mpfr_modifies a h0 h1))
@@ -88,15 +88,15 @@ inline_for_extraction val mpfr_mul_1_round: a:mpfr_ptr -> sh:mpfr_prec_t -> ax:m
 let mpfr_mul_1_round a sh ax rb sb mask rnd_mode =
     let ap = mpfr_MANT a in
     let a0 = ap.(0ul) in
-    if I32.(ax >^ mpfr_EMAX) then mpfr_overflow a rnd_mode (mpfr_SIGN a)
-    else if I32.(ax <^ mpfr_EMIN) then begin
+    if I64.(ax >^ mpfr_EMAX) then mpfr_overflow a rnd_mode (mpfr_SIGN a)
+    else if I64.(ax <^ mpfr_EMIN) then begin
         let aneg = mpfr_IS_NEG a in
-        if I32.(ax =^ mpfr_EMIN -^ 1l) && a0 =^ lognot mask &&
+        if I64.(ax =^ mpfr_EMIN -^ 1L) && a0 =^ lognot mask &&
 	   ((MPFR_RNDN? rnd_mode && rb >^ 0uL) ||
 	    (((rb |^ sb) >^ 0uL) && mpfr_IS_LIKE_RNDA rnd_mode aneg)) 
 	then mpfr_mul_1_rounding a sh ax rb sb rnd_mode
         else if MPFR_RNDN? rnd_mode &&
-	        (I32.(ax <^ mpfr_EMIN -^ 1l) ||
+	        (I64.(ax <^ mpfr_EMIN -^ 1L) ||
 		 (a0 =^ mpfr_LIMB_HIGHBIT && ((rb |^ sb) =^ 0uL)))
         then mpfr_underflow a MPFR_RNDZ (mpfr_SIGN a)
         else mpfr_underflow a rnd_mode (mpfr_SIGN a)
@@ -112,8 +112,8 @@ val mpfr_mul_1: a:mpfr_ptr -> b:mpfr_ptr -> c:mpfr_ptr ->
         length (as_struct h a).mpfr_d = 1 /\
         length (as_struct h b).mpfr_d = 1 /\ length (as_struct h c).mpfr_d = 1 /\
         (* Functional correctness *)
-        U32.v p > 0 /\ U32.v p < 64 /\ p = (as_struct h a).mpfr_prec /\
-        U32.v (as_struct h b).mpfr_prec <= 64 /\ U32.v (as_struct h c).mpfr_prec <= 64 /\
+        I64.v p < 64 /\ p = (as_struct h a).mpfr_prec /\
+        I64.v (as_struct h b).mpfr_prec <= 64 /\ I64.v (as_struct h c).mpfr_prec <= 64 /\
         mpfr_valid_cond h a /\ mpfr_reg_cond h b /\ mpfr_reg_cond h c))
     (ensures  (fun h0 t h1 -> 
         let exact = mul_exact (as_fp h0 b) (as_fp h0 c) in
@@ -132,15 +132,15 @@ let mpfr_mul_1 a b c rnd_mode p =
     let cp = mpfr_MANT c in
     let b0 = bp.(0ul) in
     let c0 = cp.(0ul) in
-    let sh = U32.(gmp_NUMB_BITS -^ p) in
-    let mask = mpfr_LIMB_MASK sh in
-    let ax = I32.(mpfr_EXP b +^ mpfr_EXP c) in
+    let sh = I64.(gmp_NUMB_BITS -^ p) in
+    let mask = mpfr_LIMB_MASK (int64_to_uint32 sh) in
+    let ax = I64.(mpfr_EXP b +^ mpfr_EXP c) in
     let a0, sb = umul_ppmm b0 c0 in
     let ax, a0, sb =
         if a0 <^ mpfr_LIMB_HIGHBIT then
-	    I32.(ax -^ 1l), (a0 <<^ 1ul) |^ (sb >>^ U32.(gmp_NUMB_BITS -^ 1ul)), sb <<^ 1ul
+	    I64.(ax -^ 1L), (a0 <<^ 1ul) |^ (sb >>^ (int64_to_uint32 I64.(gmp_NUMB_BITS -^ 1L))), sb <<^ 1ul
 	else ax, a0, sb in
-    let rb = a0 &^ (mpfr_LIMB_ONE <<^ U32.(sh -^ 1ul)) in
+    let rb = a0 &^ (mpfr_LIMB_ONE <<^ (int64_to_uint32 I64.(sh -^ 1L))) in
     let sb = sb |^ ((a0 &^ mask) ^^ rb) in
     ap.(0ul) <- a0 &^ (lognot mask);
     mpfr_SET_SIGN a (mpfr_MULT_SIGN (mpfr_SIGN b) (mpfr_SIGN c));
